Category_Set_Arithmetic/Inequality.thy
@@ -12,6 +12,15 @@ lemma leq_type[type_rule]:
   "leq : \<nat>\<^sub>c \<times>\<^sub>c \<nat>\<^sub>c \<rightarrow> \<Omega>"
   unfolding leq_def by typecheck_cfuncs
 
+definition lt :: "cfunc" where
+  "lt =
+     NOT \<circ>\<^sub>c leq \<circ>\<^sub>c
+       \<langle> right_cart_proj \<nat>\<^sub>c \<nat>\<^sub>c
+       , left_cart_proj  \<nat>\<^sub>c \<nat>\<^sub>c \<rangle>"
+
+definition lt_infix :: "cfunc \<Rightarrow> cfunc \<Rightarrow> bool" (infix "<\<^sub>\<nat>" 50) where
+  "a <\<^sub>\<nat> b = (lt \<circ>\<^sub>c \<langle>a, b\<rangle> = \<t>)"
+
 lemma leq_true_implies_exists:
   assumes m_type: "m \<in>\<^sub>c \<nat>\<^sub>c" and n_type: "n \<in>\<^sub>c \<nat>\<^sub>c"
   assumes leq_true: "leq \<circ>\<^sub>c \<langle>m, n\<rangle> = \<t>"
@@ -47,7 +56,13 @@ proof -
   then have "\<exists> k. k \<in>\<^sub>c \<nat>\<^sub>c \<and> eq_pred \<nat>\<^sub>c \<circ>\<^sub>c (add2 \<times>\<^sub>f id \<nat>\<^sub>c) \<circ>\<^sub>c \<langle>\<langle>k, m\<rangle>, n\<rangle> = \<t>"
     using associate_left_ap m_type n_type by auto
   then have "\<exists> k. k \<in>\<^sub>c \<nat>\<^sub>c \<and> eq_pred \<nat>\<^sub>c \<circ>\<^sub>c \<langle>(add2  \<circ>\<^sub>c \<langle>k, m\<rangle>), (id \<nat>\<^sub>c \<circ>\<^sub>c n)\<rangle> = \<t>"
-    by (typecheck_cfuncs, smt (verit, best) cfunc_cross_prod_comp_cfunc_prod cfunc_prod_type assms)
+  proof (rule ex_forward, auto)
+    fix k
+    assume k_type: "k \<in>\<^sub>c \<nat>\<^sub>c"
+    assume "eq_pred \<nat>\<^sub>c \<circ>\<^sub>c (add2 \<times>\<^sub>f id\<^sub>c \<nat>\<^sub>c) \<circ>\<^sub>c \<langle>\<langle>k,m\<rangle>,n\<rangle> = \<t>"
+    then show "eq_pred \<nat>\<^sub>c \<circ>\<^sub>c \<langle>add2 \<circ>\<^sub>c \<langle>k,m\<rangle>,id\<^sub>c \<nat>\<^sub>c \<circ>\<^sub>c n\<rangle> = \<t>"
+      using k_type assms by (typecheck_cfuncs, simp add: cfunc_cross_prod_comp_cfunc_prod)
+  qed
   then have "\<exists> k. k \<in>\<^sub>c \<nat>\<^sub>c \<and> eq_pred \<nat>\<^sub>c \<circ>\<^sub>c \<langle>add2 \<circ>\<^sub>c \<langle>k, m\<rangle>, n\<rangle> = \<t>"
     using id_left_unit2 n_type by auto
   then have "\<exists> k. k \<in>\<^sub>c \<nat>\<^sub>c \<and> add2 \<circ>\<^sub>c \<langle>k, m\<rangle> = n"
@@ -68,7 +83,13 @@ proof -
   then have "\<exists> k. k \<in>\<^sub>c \<nat>\<^sub>c \<and> eq_pred \<nat>\<^sub>c \<circ>\<^sub>c \<langle>(add2  \<circ>\<^sub>c \<langle>k, m\<rangle>), (id \<nat>\<^sub>c \<circ>\<^sub>c n)\<rangle> = \<t>"
     using id_left_unit2 n_type by auto
   then have "\<exists> k. k \<in>\<^sub>c \<nat>\<^sub>c \<and> eq_pred \<nat>\<^sub>c \<circ>\<^sub>c (add2 \<times>\<^sub>f id \<nat>\<^sub>c) \<circ>\<^sub>c \<langle>\<langle>k, m\<rangle>, n\<rangle> = \<t>"
-    by (typecheck_cfuncs, smt (verit, best) cfunc_cross_prod_comp_cfunc_prod cfunc_prod_type assms)
+     proof (rule ex_forward, auto)
+       fix k ka
+       assume k_type: "k \<in>\<^sub>c \<nat>\<^sub>c"
+       assume  "eq_pred \<nat>\<^sub>c \<circ>\<^sub>c \<langle>add2 \<circ>\<^sub>c \<langle>k,m\<rangle>,id\<^sub>c \<nat>\<^sub>c \<circ>\<^sub>c n\<rangle> = \<t>"
+       then show "eq_pred \<nat>\<^sub>c \<circ>\<^sub>c (add2 \<times>\<^sub>f id\<^sub>c \<nat>\<^sub>c) \<circ>\<^sub>c \<langle>\<langle>k,m\<rangle>,n\<rangle> = \<t>"
+         using k_type assms by (typecheck_cfuncs, simp add:  cfunc_cross_prod_comp_cfunc_prod)
+     qed
   then have "\<exists> k. k \<in>\<^sub>c \<nat>\<^sub>c \<and>  eq_pred \<nat>\<^sub>c \<circ>\<^sub>c (add2 \<times>\<^sub>f id \<nat>\<^sub>c) \<circ>\<^sub>c associate_left \<nat>\<^sub>c \<nat>\<^sub>c \<nat>\<^sub>c \<circ>\<^sub>c \<langle>k, \<langle>m, n\<rangle>\<rangle> = \<t>"
     using associate_left_ap m_type n_type by auto
   then have "\<exists> k. k \<in>\<^sub>c \<nat>\<^sub>c \<and>  eq_pred \<nat>\<^sub>c \<circ>\<^sub>c (add2 \<times>\<^sub>f id \<nat>\<^sub>c) \<circ>\<^sub>c associate_left \<nat>\<^sub>c \<nat>\<^sub>c \<nat>\<^sub>c \<circ>\<^sub>c \<langle>id \<nat>\<^sub>c, \<langle>m, n\<rangle> \<circ>\<^sub>c \<beta>\<^bsub>\<nat>\<^sub>c\<^esub>\<rangle> \<circ>\<^sub>c k = \<t>"
@@ -97,6 +118,9 @@ proof -
     using m_type n_type comp_associative2 unfolding leq_def by (typecheck_cfuncs, auto)
 qed
 
+
+
+
 lemma add_monotonic:
   assumes m_type: "m \<in>\<^sub>c \<nat>\<^sub>c" and n_type: "n \<in>\<^sub>c \<nat>\<^sub>c" and u_type: "u \<in>\<^sub>c \<nat>\<^sub>c" and v_type: "v \<in>\<^sub>c \<nat>\<^sub>c"
   assumes m_leq_n: "leq \<circ>\<^sub>c \<langle>m, n\<rangle> = \<t>" 
@@ -112,6 +136,8 @@ proof -
   show "leq \<circ>\<^sub>c \<langle>m +\<^sub>\<nat> u, n +\<^sub>\<nat> v\<rangle> = \<t>"
     by (metis add_type combined_Eqns exists_implies_leq_true m_type u_type)
 qed
+
+
 
 lemma leq_transitivity:
   assumes m_type: "m \<in>\<^sub>c \<nat>\<^sub>c" and n_type: "n \<in>\<^sub>c \<nat>\<^sub>c" and p_type: "p \<in>\<^sub>c \<nat>\<^sub>c"
@@ -133,7 +159,11 @@ proof -
      using add_type combined_Eqn j_num k_num by blast
    then show "leq \<circ>\<^sub>c \<langle>m, p\<rangle> = \<t>"
      by (simp add: exists_implies_leq_true m_type p_type)
-qed
+ qed
+
+  
+
+
 
 lemma lqe_antisymmetry:
   assumes m_type: "m \<in>\<^sub>c \<nat>\<^sub>c" and n_type: "n \<in>\<^sub>c \<nat>\<^sub>c"
@@ -167,10 +197,17 @@ proof -
     using add_respects_zero_on_left k_def n_type by blast
 qed
 
+
+
+
+
+
+
 lemma zero_is_smallest:
   assumes "n \<in>\<^sub>c \<nat>\<^sub>c"
   shows "leq \<circ>\<^sub>c\<langle>zero ,n\<rangle> = \<t>"
   using add_respects_zero_on_right assms exists_implies_leq_true zero_type by blast
+
 
 lemma fewer_is_less: 
   assumes "m \<in>\<^sub>c \<nat>\<^sub>c" 
@@ -178,23 +215,44 @@ lemma fewer_is_less:
   assumes "k \<in>\<^sub>c \<nat>\<^sub>c"
   assumes "m +\<^sub>\<nat> k \<le>\<^sub>\<nat> n"
   shows "m \<le>\<^sub>\<nat> n"
-  using assms unfolding leq_infix_def by (typecheck_cfuncs, metis add_commutes add_type exists_implies_leq_true leq_infix_def leq_transitivity)
+  using assms unfolding leq_infix_def by (typecheck_cfuncs, metis add_commutes add_type assms(3) exists_implies_leq_true leq_infix_def leq_transitivity)
+
+
+
+
+
 
 lemma lqe_connexity:
-  assumes m_type[type_rule]: "m \<in>\<^sub>c \<nat>\<^sub>c" and n_type[type_rule]: "n \<in>\<^sub>c \<nat>\<^sub>c"
+  assumes m_type: "m \<in>\<^sub>c \<nat>\<^sub>c" and n_type: "n \<in>\<^sub>c \<nat>\<^sub>c"
   shows "(leq \<circ>\<^sub>c \<langle>n, m\<rangle> = \<t>) \<or> (leq \<circ>\<^sub>c \<langle>m, n\<rangle> = \<t>)"
-proof - 
+proof-
   have main_result: "(OR \<circ>\<^sub>c \<langle>
 leq \<circ>\<^sub>c \<langle>left_cart_proj \<nat>\<^sub>c \<nat>\<^sub>c, right_cart_proj \<nat>\<^sub>c \<nat>\<^sub>c\<rangle>,
 leq \<circ>\<^sub>c \<langle>right_cart_proj \<nat>\<^sub>c \<nat>\<^sub>c, left_cart_proj \<nat>\<^sub>c \<nat>\<^sub>c\<rangle>
 \<rangle>)\<^sup>\<sharp> = (\<t> \<circ>\<^sub>c \<beta>\<^bsub>\<nat>\<^sub>c\<times>\<^sub>c\<nat>\<^sub>c\<^esub>)\<^sup>\<sharp>"
-  proof(etcs_rule natural_number_object_func_unique[where X="\<Omega>\<^bsup>\<nat>\<^sub>c\<^esup>", where f = "id (\<Omega>\<^bsup>\<nat>\<^sub>c\<^esup>)"])
+  proof(rule natural_number_object_func_unique[where X="\<Omega>\<^bsup>\<nat>\<^sub>c\<^esup>", where f = "id (\<Omega>\<^bsup>\<nat>\<^sub>c\<^esup>)" ])
+    show type_fact1: "(OR \<circ>\<^sub>c \<langle>leq \<circ>\<^sub>c\<langle>left_cart_proj \<nat>\<^sub>c \<nat>\<^sub>c,right_cart_proj \<nat>\<^sub>c \<nat>\<^sub>c\<rangle>,leq \<circ>\<^sub>c \<langle>right_cart_proj \<nat>\<^sub>c \<nat>\<^sub>c,left_cart_proj \<nat>\<^sub>c \<nat>\<^sub>c\<rangle>\<rangle>)\<^sup>\<sharp> : \<nat>\<^sub>c \<rightarrow> \<Omega>\<^bsup>\<nat>\<^sub>c\<^esup>"
+      by typecheck_cfuncs
+    show type_fact2: "(\<t> \<circ>\<^sub>c \<beta>\<^bsub>\<nat>\<^sub>c \<times>\<^sub>c \<nat>\<^sub>c\<^esub>)\<^sup>\<sharp> : \<nat>\<^sub>c \<rightarrow> \<Omega>\<^bsup>\<nat>\<^sub>c\<^esup>"
+      by typecheck_cfuncs
+    have type_fact3: "id\<^sub>c \<nat>\<^sub>c \<times>\<^sub>f (\<t> \<circ>\<^sub>c \<beta>\<^bsub>\<nat>\<^sub>c \<times>\<^sub>c \<nat>\<^sub>c\<^esub>)\<^sup>\<sharp> \<circ>\<^sub>c zero : \<nat>\<^sub>c\<times>\<^sub>c \<one> \<rightarrow> \<nat>\<^sub>c\<times>\<^sub>c\<Omega>\<^bsup>\<nat>\<^sub>c\<^esup>"
+      by typecheck_cfuncs
+    show type_fact3: "id\<^sub>c (\<Omega>\<^bsup>\<nat>\<^sub>c\<^esup>) : \<Omega>\<^bsup>\<nat>\<^sub>c\<^esup> \<rightarrow> \<Omega>\<^bsup>\<nat>\<^sub>c\<^esup>"
+      by typecheck_cfuncs
     show eqn_1: "(OR \<circ>\<^sub>c \<langle>leq \<circ>\<^sub>c \<langle>left_cart_proj \<nat>\<^sub>c \<nat>\<^sub>c,right_cart_proj \<nat>\<^sub>c \<nat>\<^sub>c\<rangle>,leq \<circ>\<^sub>c \<langle>right_cart_proj \<nat>\<^sub>c \<nat>\<^sub>c,left_cart_proj \<nat>\<^sub>c \<nat>\<^sub>c\<rangle>\<rangle>)\<^sup>\<sharp> \<circ>\<^sub>c zero =
             (\<t> \<circ>\<^sub>c \<beta>\<^bsub>\<nat>\<^sub>c \<times>\<^sub>c \<nat>\<^sub>c\<^esub>)\<^sup>\<sharp> \<circ>\<^sub>c zero"
-    proof(etcs_rule same_evals_equal[where Z = "\<one>", where X=\<Omega>, where A="\<nat>\<^sub>c"])
+    proof(rule same_evals_equal[where Z = "\<one>", where X=\<Omega>, where A="\<nat>\<^sub>c"])
+      show type_fact5: "(OR \<circ>\<^sub>c \<langle>leq \<circ>\<^sub>c \<langle>left_cart_proj \<nat>\<^sub>c \<nat>\<^sub>c,right_cart_proj \<nat>\<^sub>c \<nat>\<^sub>c\<rangle>, leq \<circ>\<^sub>c \<langle>right_cart_proj \<nat>\<^sub>c \<nat>\<^sub>c,left_cart_proj \<nat>\<^sub>c \<nat>\<^sub>c\<rangle>\<rangle>)\<^sup>\<sharp> \<circ>\<^sub>c zero \<in>\<^sub>c \<Omega>\<^bsup>\<nat>\<^sub>c\<^esup>"
+        by typecheck_cfuncs
+      show type_fact6: "(\<t> \<circ>\<^sub>c \<beta>\<^bsub>\<nat>\<^sub>c \<times>\<^sub>c \<nat>\<^sub>c\<^esub>)\<^sup>\<sharp> \<circ>\<^sub>c zero \<in>\<^sub>c \<Omega>\<^bsup>\<nat>\<^sub>c\<^esup>"
+        by typecheck_cfuncs
       show eqn_2: "eval_func \<Omega> \<nat>\<^sub>c \<circ>\<^sub>c id\<^sub>c \<nat>\<^sub>c \<times>\<^sub>f (OR \<circ>\<^sub>c \<langle>leq \<circ>\<^sub>c \<langle>left_cart_proj \<nat>\<^sub>c \<nat>\<^sub>c,right_cart_proj \<nat>\<^sub>c \<nat>\<^sub>c\<rangle>,leq \<circ>\<^sub>c \<langle>right_cart_proj \<nat>\<^sub>c \<nat>\<^sub>c,left_cart_proj \<nat>\<^sub>c \<nat>\<^sub>c\<rangle>\<rangle>)\<^sup>\<sharp> \<circ>\<^sub>c zero =
             eval_func \<Omega> \<nat>\<^sub>c \<circ>\<^sub>c id\<^sub>c \<nat>\<^sub>c \<times>\<^sub>f (\<t> \<circ>\<^sub>c \<beta>\<^bsub>\<nat>\<^sub>c \<times>\<^sub>c \<nat>\<^sub>c\<^esub>)\<^sup>\<sharp> \<circ>\<^sub>c zero"
-      proof(etcs_rule one_separator[where X="\<nat>\<^sub>c\<times>\<^sub>c \<one>", where Y = \<Omega>])
+      proof(rule one_separator[where X="\<nat>\<^sub>c\<times>\<^sub>c \<one>", where Y = \<Omega>])
+        show type_fact7: "eval_func \<Omega> \<nat>\<^sub>c \<circ>\<^sub>c id\<^sub>c \<nat>\<^sub>c \<times>\<^sub>f (OR \<circ>\<^sub>c \<langle>leq \<circ>\<^sub>c \<langle>left_cart_proj \<nat>\<^sub>c \<nat>\<^sub>c,right_cart_proj \<nat>\<^sub>c \<nat>\<^sub>c\<rangle>, leq \<circ>\<^sub>c \<langle>right_cart_proj \<nat>\<^sub>c \<nat>\<^sub>c,left_cart_proj \<nat>\<^sub>c \<nat>\<^sub>c\<rangle>\<rangle>)\<^sup>\<sharp> \<circ>\<^sub>c            zero : \<nat>\<^sub>c \<times>\<^sub>c \<one> \<rightarrow> \<Omega>"
+          by typecheck_cfuncs
+        show type_fact8: "eval_func \<Omega> \<nat>\<^sub>c \<circ>\<^sub>c  id\<^sub>c \<nat>\<^sub>c \<times>\<^sub>f (\<t> \<circ>\<^sub>c \<beta>\<^bsub>\<nat>\<^sub>c \<times>\<^sub>c \<nat>\<^sub>c\<^esub>)\<^sup>\<sharp> \<circ>\<^sub>c zero : \<nat>\<^sub>c \<times>\<^sub>c \<one> \<rightarrow> \<Omega>"
+          by typecheck_cfuncs
         show "\<And>x. x \<in>\<^sub>c \<nat>\<^sub>c \<times>\<^sub>c \<one> \<Longrightarrow>
              (eval_func \<Omega> \<nat>\<^sub>c \<circ>\<^sub>c id\<^sub>c \<nat>\<^sub>c \<times>\<^sub>f (OR \<circ>\<^sub>c
              \<langle>leq \<circ>\<^sub>c \<langle>left_cart_proj \<nat>\<^sub>c \<nat>\<^sub>c,right_cart_proj \<nat>\<^sub>c \<nat>\<^sub>c\<rangle>,
@@ -209,7 +267,7 @@ leq \<circ>\<^sub>c \<langle>right_cart_proj \<nat>\<^sub>c \<nat>\<^sub>c, left
           proof - 
             have "(eval_func \<Omega> \<nat>\<^sub>c \<circ>\<^sub>c id\<^sub>c \<nat>\<^sub>c \<times>\<^sub>f (\<t> \<circ>\<^sub>c \<beta>\<^bsub>\<nat>\<^sub>c \<times>\<^sub>c \<nat>\<^sub>c\<^esub>)\<^sup>\<sharp> \<circ>\<^sub>c zero) \<circ>\<^sub>c x = 
                   (eval_func \<Omega> \<nat>\<^sub>c \<circ>\<^sub>c id\<^sub>c \<nat>\<^sub>c \<times>\<^sub>f (\<t> \<circ>\<^sub>c \<beta>\<^bsub>\<nat>\<^sub>c \<times>\<^sub>c \<nat>\<^sub>c\<^esub>)\<^sup>\<sharp>) \<circ>\<^sub>c (id\<^sub>c \<nat>\<^sub>c \<times>\<^sub>f zero) \<circ>\<^sub>c x"
-              by (typecheck_cfuncs, smt cfunc_type_def comp_associative inv_transpose_func_def3 inv_transpose_of_composition x_type)
+              by (typecheck_cfuncs, simp add: comp_associative2 identity_distributes_across_composition)
             also have "... = (\<t> \<circ>\<^sub>c \<beta>\<^bsub>\<nat>\<^sub>c \<times>\<^sub>c \<nat>\<^sub>c\<^esub>) \<circ>\<^sub>c (id\<^sub>c \<nat>\<^sub>c \<times>\<^sub>f zero) \<circ>\<^sub>c \<langle>j,id \<one>\<rangle>"
               by (typecheck_cfuncs, simp add: j_def transpose_func_def)
             also have "... = (\<t> \<circ>\<^sub>c \<beta>\<^bsub>\<nat>\<^sub>c \<times>\<^sub>c \<nat>\<^sub>c\<^esub>) \<circ>\<^sub>c \<langle>id\<^sub>c \<nat>\<^sub>c \<circ>\<^sub>c j,zero \<circ>\<^sub>c id \<one>\<rangle>"
@@ -220,7 +278,8 @@ leq \<circ>\<^sub>c \<langle>right_cart_proj \<nat>\<^sub>c \<nat>\<^sub>c, left
               by (typecheck_cfuncs, metis id_right_unit2 terminal_func_unique)
             then show ?thesis
               by (simp add: calculation)
-          qed          
+          qed
+          
           have eqn_LHS: "(eval_func \<Omega> \<nat>\<^sub>c \<circ>\<^sub>c  id\<^sub>c \<nat>\<^sub>c \<times>\<^sub>f
             (OR \<circ>\<^sub>c \<langle>leq \<circ>\<^sub>c \<langle>left_cart_proj \<nat>\<^sub>c \<nat>\<^sub>c,right_cart_proj \<nat>\<^sub>c \<nat>\<^sub>c\<rangle>,
                     leq \<circ>\<^sub>c\<langle>right_cart_proj \<nat>\<^sub>c \<nat>\<^sub>c,left_cart_proj \<nat>\<^sub>c \<nat>\<^sub>c\<rangle>\<rangle>)\<^sup>\<sharp> \<circ>\<^sub>c zero) \<circ>\<^sub>c x = \<t>"
@@ -232,7 +291,7 @@ leq \<circ>\<^sub>c \<langle>right_cart_proj \<nat>\<^sub>c \<nat>\<^sub>c, left
             (OR \<circ>\<^sub>c \<langle>leq \<circ>\<^sub>c \<langle>left_cart_proj \<nat>\<^sub>c \<nat>\<^sub>c,right_cart_proj \<nat>\<^sub>c \<nat>\<^sub>c\<rangle>,
                     leq \<circ>\<^sub>c\<langle>right_cart_proj \<nat>\<^sub>c \<nat>\<^sub>c,left_cart_proj \<nat>\<^sub>c \<nat>\<^sub>c\<rangle>\<rangle>)\<^sup>\<sharp>)  \<circ>\<^sub>c
                  (id\<^sub>c \<nat>\<^sub>c \<times>\<^sub>f zero) \<circ>\<^sub>c x"
-                by (typecheck_cfuncs, smt cfunc_type_def comp_associative inv_transpose_func_def3 inv_transpose_of_composition x_type)
+                by (typecheck_cfuncs, simp add: comp_associative2 identity_distributes_across_composition)
               also have "... = OR \<circ>\<^sub>c \<langle>leq \<circ>\<^sub>c \<langle>left_cart_proj \<nat>\<^sub>c \<nat>\<^sub>c,right_cart_proj \<nat>\<^sub>c \<nat>\<^sub>c\<rangle>,
                     leq \<circ>\<^sub>c\<langle>right_cart_proj \<nat>\<^sub>c \<nat>\<^sub>c,left_cart_proj \<nat>\<^sub>c \<nat>\<^sub>c\<rangle>\<rangle> \<circ>\<^sub>c
                  (id\<^sub>c \<nat>\<^sub>c \<times>\<^sub>f zero) \<circ>\<^sub>c x"
@@ -266,10 +325,18 @@ leq \<circ>\<^sub>c \<langle>right_cart_proj \<nat>\<^sub>c \<nat>\<^sub>c, left
       qed
     show "(\<t> \<circ>\<^sub>c \<beta>\<^bsub>\<nat>\<^sub>c \<times>\<^sub>c \<nat>\<^sub>c\<^esub>)\<^sup>\<sharp> \<circ>\<^sub>c successor =
     id\<^sub>c (\<Omega>\<^bsup>\<nat>\<^sub>c\<^esup>) \<circ>\<^sub>c (\<t> \<circ>\<^sub>c \<beta>\<^bsub>\<nat>\<^sub>c \<times>\<^sub>c \<nat>\<^sub>c\<^esub>)\<^sup>\<sharp>"
-      proof(etcs_rule same_evals_equal[where Z = "\<nat>\<^sub>c", where X = \<Omega>,where A = "\<nat>\<^sub>c"])
+      proof(rule same_evals_equal[where Z = "\<nat>\<^sub>c", where X = \<Omega>,where A = "\<nat>\<^sub>c"])
+        show type_fact9: "(\<t> \<circ>\<^sub>c \<beta>\<^bsub>\<nat>\<^sub>c \<times>\<^sub>c \<nat>\<^sub>c\<^esub>)\<^sup>\<sharp> \<circ>\<^sub>c successor : \<nat>\<^sub>c \<rightarrow> \<Omega>\<^bsup>\<nat>\<^sub>c\<^esup>"
+          by typecheck_cfuncs
+        show type_fact10: "id\<^sub>c (\<Omega>\<^bsup>\<nat>\<^sub>c\<^esup>) \<circ>\<^sub>c (\<t> \<circ>\<^sub>c \<beta>\<^bsub>\<nat>\<^sub>c \<times>\<^sub>c \<nat>\<^sub>c\<^esub>)\<^sup>\<sharp> : \<nat>\<^sub>c \<rightarrow> \<Omega>\<^bsup>\<nat>\<^sub>c\<^esup>"
+          by typecheck_cfuncs
         show "eval_func \<Omega> \<nat>\<^sub>c \<circ>\<^sub>c id\<^sub>c \<nat>\<^sub>c \<times>\<^sub>f (\<t> \<circ>\<^sub>c \<beta>\<^bsub>\<nat>\<^sub>c \<times>\<^sub>c \<nat>\<^sub>c\<^esub>)\<^sup>\<sharp> \<circ>\<^sub>c successor =
     eval_func \<Omega> \<nat>\<^sub>c \<circ>\<^sub>c id\<^sub>c \<nat>\<^sub>c \<times>\<^sub>f id\<^sub>c (\<Omega>\<^bsup>\<nat>\<^sub>c\<^esup>) \<circ>\<^sub>c (\<t> \<circ>\<^sub>c \<beta>\<^bsub>\<nat>\<^sub>c \<times>\<^sub>c \<nat>\<^sub>c\<^esub>)\<^sup>\<sharp>"
-        proof(etcs_rule one_separator[where X="\<nat>\<^sub>c\<times>\<^sub>c\<nat>\<^sub>c", where Y = \<Omega>])
+        proof(rule one_separator[where X="\<nat>\<^sub>c\<times>\<^sub>c\<nat>\<^sub>c", where Y = \<Omega>])
+          show type_fact11: "eval_func \<Omega> \<nat>\<^sub>c \<circ>\<^sub>c id\<^sub>c \<nat>\<^sub>c \<times>\<^sub>f (\<t> \<circ>\<^sub>c \<beta>\<^bsub>\<nat>\<^sub>c \<times>\<^sub>c \<nat>\<^sub>c\<^esub>)\<^sup>\<sharp> \<circ>\<^sub>c successor : \<nat>\<^sub>c \<times>\<^sub>c \<nat>\<^sub>c \<rightarrow> \<Omega>"
+            by typecheck_cfuncs
+          show type_fact12: "eval_func \<Omega> \<nat>\<^sub>c \<circ>\<^sub>c id\<^sub>c \<nat>\<^sub>c \<times>\<^sub>f id\<^sub>c (\<Omega>\<^bsup>\<nat>\<^sub>c\<^esup>) \<circ>\<^sub>c (\<t> \<circ>\<^sub>c \<beta>\<^bsub>\<nat>\<^sub>c \<times>\<^sub>c \<nat>\<^sub>c\<^esub>)\<^sup>\<sharp> : \<nat>\<^sub>c \<times>\<^sub>c \<nat>\<^sub>c \<rightarrow> \<Omega>"
+            by typecheck_cfuncs
           show "\<And>x. x \<in>\<^sub>c \<nat>\<^sub>c \<times>\<^sub>c \<nat>\<^sub>c \<Longrightarrow>
          (eval_func \<Omega> \<nat>\<^sub>c \<circ>\<^sub>c id\<^sub>c \<nat>\<^sub>c \<times>\<^sub>f (\<t> \<circ>\<^sub>c \<beta>\<^bsub>\<nat>\<^sub>c \<times>\<^sub>c \<nat>\<^sub>c\<^esub>)\<^sup>\<sharp> \<circ>\<^sub>c successor) \<circ>\<^sub>c  x =
          (eval_func \<Omega> \<nat>\<^sub>c \<circ>\<^sub>c id\<^sub>c \<nat>\<^sub>c \<times>\<^sub>f id\<^sub>c (\<Omega>\<^bsup>\<nat>\<^sub>c\<^esup>) \<circ>\<^sub>c (\<t> \<circ>\<^sub>c \<beta>\<^bsub>\<nat>\<^sub>c \<times>\<^sub>c \<nat>\<^sub>c\<^esub>)\<^sup>\<sharp>) \<circ>\<^sub>cx"
@@ -278,11 +345,14 @@ leq \<circ>\<^sub>c \<langle>right_cart_proj \<nat>\<^sub>c \<nat>\<^sub>c, left
             assume x_def: "x \<in>\<^sub>c \<nat>\<^sub>c \<times>\<^sub>c \<nat>\<^sub>c"
            
             show "(eval_func \<Omega> \<nat>\<^sub>c \<circ>\<^sub>c id\<^sub>c \<nat>\<^sub>c \<times>\<^sub>f (\<t> \<circ>\<^sub>c \<beta>\<^bsub>\<nat>\<^sub>c \<times>\<^sub>c \<nat>\<^sub>c\<^esub>)\<^sup>\<sharp> \<circ>\<^sub>c successor) \<circ>\<^sub>c  x =
-                  (eval_func \<Omega> \<nat>\<^sub>c \<circ>\<^sub>c id\<^sub>c \<nat>\<^sub>c \<times>\<^sub>f id\<^sub>c (\<Omega>\<^bsup>\<nat>\<^sub>c\<^esup>) \<circ>\<^sub>c (\<t> \<circ>\<^sub>c \<beta>\<^bsub>\<nat>\<^sub>c \<times>\<^sub>c \<nat>\<^sub>c\<^esub>)\<^sup>\<sharp>) \<circ>\<^sub>cx"          
+                  (eval_func \<Omega> \<nat>\<^sub>c \<circ>\<^sub>c id\<^sub>c \<nat>\<^sub>c \<times>\<^sub>f id\<^sub>c (\<Omega>\<^bsup>\<nat>\<^sub>c\<^esup>) \<circ>\<^sub>c (\<t> \<circ>\<^sub>c \<beta>\<^bsub>\<nat>\<^sub>c \<times>\<^sub>c \<nat>\<^sub>c\<^esub>)\<^sup>\<sharp>) \<circ>\<^sub>cx"
+            
+
             proof - 
               have calc1: "(eval_func \<Omega> \<nat>\<^sub>c \<circ>\<^sub>c id\<^sub>c \<nat>\<^sub>c \<times>\<^sub>f (\<t> \<circ>\<^sub>c \<beta>\<^bsub>\<nat>\<^sub>c \<times>\<^sub>c \<nat>\<^sub>c\<^esub>)\<^sup>\<sharp> \<circ>\<^sub>c successor) \<circ>\<^sub>c  x =
                            (eval_func \<Omega> \<nat>\<^sub>c \<circ>\<^sub>c id\<^sub>c \<nat>\<^sub>c \<times>\<^sub>f (\<t> \<circ>\<^sub>c \<beta>\<^bsub>\<nat>\<^sub>c \<times>\<^sub>c \<nat>\<^sub>c\<^esub>)\<^sup>\<sharp>)\<circ>\<^sub>c (id\<^sub>c \<nat>\<^sub>c \<times>\<^sub>f successor) \<circ>\<^sub>c  x"
-                by (typecheck_cfuncs, smt cfunc_type_def comp_associative inv_transpose_func_def3 inv_transpose_of_composition x_def)     
+                by (typecheck_cfuncs,
+                smt (verit, best) comp_associative2 sharp_comp terminal_func_comp transpose_func_def x_def)
               also have "... = (\<t> \<circ>\<^sub>c \<beta>\<^bsub>\<nat>\<^sub>c \<times>\<^sub>c \<nat>\<^sub>c\<^esub>) \<circ>\<^sub>c (id\<^sub>c \<nat>\<^sub>c \<times>\<^sub>f successor) \<circ>\<^sub>c  x"
                 using transpose_func_def by (typecheck_cfuncs, auto)
               also have "... = \<t> \<circ>\<^sub>c (\<beta>\<^bsub>\<nat>\<^sub>c \<times>\<^sub>c \<nat>\<^sub>c\<^esub> \<circ>\<^sub>c (id\<^sub>c \<nat>\<^sub>c \<times>\<^sub>f successor) \<circ>\<^sub>c  x)"
@@ -310,11 +380,18 @@ leq \<circ>\<^sub>c \<langle>right_cart_proj \<nat>\<^sub>c \<nat>\<^sub>c, left
           qed
         qed
       qed
+
+      
+
       show "(OR \<circ>\<^sub>c \<langle>leq \<circ>\<^sub>c \<langle>left_cart_proj \<nat>\<^sub>c \<nat>\<^sub>c,right_cart_proj \<nat>\<^sub>c \<nat>\<^sub>c\<rangle>,
                    leq \<circ>\<^sub>c \<langle>right_cart_proj \<nat>\<^sub>c \<nat>\<^sub>c,left_cart_proj \<nat>\<^sub>c \<nat>\<^sub>c\<rangle>\<rangle>)\<^sup>\<sharp> \<circ>\<^sub>c  successor =
     id\<^sub>c (\<Omega>\<^bsup>\<nat>\<^sub>c\<^esup>) \<circ>\<^sub>c (OR \<circ>\<^sub>c \<langle>leq \<circ>\<^sub>c \<langle>left_cart_proj \<nat>\<^sub>c \<nat>\<^sub>c,right_cart_proj \<nat>\<^sub>c \<nat>\<^sub>c\<rangle>,
                           leq \<circ>\<^sub>c \<langle>right_cart_proj \<nat>\<^sub>c \<nat>\<^sub>c,left_cart_proj \<nat>\<^sub>c \<nat>\<^sub>c\<rangle>\<rangle>)\<^sup>\<sharp>"
-        proof(etcs_rule same_evals_equal[where Z="\<nat>\<^sub>c", where X=\<Omega>, where A ="\<nat>\<^sub>c" ])
+        proof(rule same_evals_equal[where Z="\<nat>\<^sub>c", where X=\<Omega>, where A ="\<nat>\<^sub>c" ])
+          show type_fact13: "(OR \<circ>\<^sub>c \<langle>leq \<circ>\<^sub>c\<langle>left_cart_proj \<nat>\<^sub>c \<nat>\<^sub>c,right_cart_proj \<nat>\<^sub>c \<nat>\<^sub>c\<rangle>, leq \<circ>\<^sub>c\<langle>right_cart_proj \<nat>\<^sub>c \<nat>\<^sub>c,left_cart_proj \<nat>\<^sub>c \<nat>\<^sub>c\<rangle>\<rangle>)\<^sup>\<sharp> \<circ>\<^sub>c    successor : \<nat>\<^sub>c \<rightarrow> \<Omega>\<^bsup>\<nat>\<^sub>c\<^esup>"
+            by typecheck_cfuncs
+          show type_fact14: "id\<^sub>c (\<Omega>\<^bsup>\<nat>\<^sub>c\<^esup>) \<circ>\<^sub>c (OR \<circ>\<^sub>c \<langle>leq \<circ>\<^sub>c \<langle>left_cart_proj \<nat>\<^sub>c \<nat>\<^sub>c,right_cart_proj \<nat>\<^sub>c \<nat>\<^sub>c\<rangle>, leq \<circ>\<^sub>c \<langle>right_cart_proj \<nat>\<^sub>c \<nat>\<^sub>c,left_cart_proj \<nat>\<^sub>c \<nat>\<^sub>c\<rangle>\<rangle>)\<^sup>\<sharp> : \<nat>\<^sub>c \<rightarrow> \<Omega>\<^bsup>\<nat>\<^sub>c\<^esup>"
+            by typecheck_cfuncs
           show "eval_func \<Omega> \<nat>\<^sub>c \<circ>\<^sub>c
     id\<^sub>c \<nat>\<^sub>c \<times>\<^sub>f
     (OR \<circ>\<^sub>c \<langle>leq \<circ>\<^sub>c \<langle>left_cart_proj \<nat>\<^sub>c \<nat>\<^sub>c,right_cart_proj \<nat>\<^sub>c \<nat>\<^sub>c\<rangle>,
@@ -323,8 +400,11 @@ leq \<circ>\<^sub>c \<langle>right_cart_proj \<nat>\<^sub>c \<nat>\<^sub>c, left
     eval_func \<Omega> \<nat>\<^sub>c \<circ>\<^sub>c id\<^sub>c \<nat>\<^sub>c \<times>\<^sub>f id\<^sub>c (\<Omega>\<^bsup>\<nat>\<^sub>c\<^esup>) \<circ>\<^sub>c
     (OR \<circ>\<^sub>c \<langle>leq \<circ>\<^sub>c \<langle>left_cart_proj \<nat>\<^sub>c \<nat>\<^sub>c,right_cart_proj \<nat>\<^sub>c \<nat>\<^sub>c\<rangle>,
            leq \<circ>\<^sub>c \<langle>right_cart_proj \<nat>\<^sub>c \<nat>\<^sub>c,left_cart_proj \<nat>\<^sub>c \<nat>\<^sub>c\<rangle>\<rangle>)\<^sup>\<sharp>"
-          proof(etcs_rule one_separator[where X = "\<nat>\<^sub>c\<times>\<^sub>c\<nat>\<^sub>c", where Y = \<Omega>])
-          
+          proof(rule one_separator[where X = "\<nat>\<^sub>c\<times>\<^sub>c\<nat>\<^sub>c", where Y = \<Omega>])
+            show type_fact15: "eval_func \<Omega> \<nat>\<^sub>c \<circ>\<^sub>c id\<^sub>c \<nat>\<^sub>c \<times>\<^sub>f  (OR \<circ>\<^sub>c \<langle>leq \<circ>\<^sub>c \<langle>left_cart_proj \<nat>\<^sub>c \<nat>\<^sub>c,right_cart_proj \<nat>\<^sub>c \<nat>\<^sub>c\<rangle>, leq \<circ>\<^sub>c \<langle>right_cart_proj \<nat>\<^sub>c \<nat>\<^sub>c,left_cart_proj \<nat>\<^sub>c \<nat>\<^sub>c\<rangle>\<rangle>)\<^sup>\<sharp> \<circ>\<^sub>c successor : \<nat>\<^sub>c \<times>\<^sub>c \<nat>\<^sub>c \<rightarrow> \<Omega>"
+              by typecheck_cfuncs
+            show "eval_func \<Omega> \<nat>\<^sub>c \<circ>\<^sub>c id\<^sub>c \<nat>\<^sub>c \<times>\<^sub>f id\<^sub>c (\<Omega>\<^bsup>\<nat>\<^sub>c\<^esup>) \<circ>\<^sub>c (OR \<circ>\<^sub>c \<langle>leq \<circ>\<^sub>c \<langle>left_cart_proj \<nat>\<^sub>c \<nat>\<^sub>c,right_cart_proj \<nat>\<^sub>c \<nat>\<^sub>c\<rangle>, leq \<circ>\<^sub>c \<langle>right_cart_proj \<nat>\<^sub>c \<nat>\<^sub>c,left_cart_proj \<nat>\<^sub>c \<nat>\<^sub>c\<rangle>\<rangle>)\<^sup>\<sharp> : \<nat>\<^sub>c \<times>\<^sub>c \<nat>\<^sub>c \<rightarrow> \<Omega>"
+              by typecheck_cfuncs
             show "\<And>x. x \<in>\<^sub>c \<nat>\<^sub>c \<times>\<^sub>c \<nat>\<^sub>c \<Longrightarrow>
          (eval_func \<Omega> \<nat>\<^sub>c \<circ>\<^sub>c id\<^sub>c \<nat>\<^sub>c \<times>\<^sub>f
           (OR \<circ>\<^sub>c \<langle>leq \<circ>\<^sub>c \<langle>left_cart_proj \<nat>\<^sub>c \<nat>\<^sub>c,right_cart_proj \<nat>\<^sub>c \<nat>\<^sub>c\<rangle>,
@@ -343,20 +423,23 @@ leq \<circ>\<^sub>c \<langle>right_cart_proj \<nat>\<^sub>c \<nat>\<^sub>c, left
               obtain m where m_def: "n \<in>\<^sub>c \<nat>\<^sub>c \<and> m \<in>\<^sub>c \<nat>\<^sub>c \<and> x = \<langle>n,m\<rangle>"
                 using n_def by blast
 
+
               have nsm_type: "\<langle>n,successor \<circ>\<^sub>c m\<rangle> \<in>\<^sub>c \<nat>\<^sub>c \<times>\<^sub>c \<nat>\<^sub>c"
                 by (simp add: cfunc_prod_type m_def succ_n_type)
               have smn_type: "\<langle>successor \<circ>\<^sub>c m,n\<rangle> \<in>\<^sub>c \<nat>\<^sub>c \<times>\<^sub>c \<nat>\<^sub>c"
                 by (simp add: cfunc_prod_type m_def succ_n_type)
 
               have "(eval_func \<Omega> \<nat>\<^sub>c \<circ>\<^sub>c id\<^sub>c \<nat>\<^sub>c \<times>\<^sub>f
-                    (OR \<circ>\<^sub>c \<langle>leq \<circ>\<^sub>c \<langle>left_cart_proj \<nat>\<^sub>c \<nat>\<^sub>c,right_cart_proj \<nat>\<^sub>c \<nat>\<^sub>c\<rangle>,
-                           leq \<circ>\<^sub>c \<langle>right_cart_proj \<nat>\<^sub>c \<nat>\<^sub>c,left_cart_proj \<nat>\<^sub>c \<nat>\<^sub>c\<rangle>\<rangle>)\<^sup>\<sharp> \<circ>\<^sub>c successor) \<circ>\<^sub>c \<langle>n,m\<rangle> =
-                    (eval_func \<Omega> \<nat>\<^sub>c \<circ>\<^sub>c id\<^sub>c \<nat>\<^sub>c \<times>\<^sub>f id\<^sub>c (\<Omega>\<^bsup>\<nat>\<^sub>c\<^esup>) \<circ>\<^sub>c
-                    (OR \<circ>\<^sub>c \<langle>leq \<circ>\<^sub>c \<langle>left_cart_proj \<nat>\<^sub>c \<nat>\<^sub>c,right_cart_proj \<nat>\<^sub>c \<nat>\<^sub>c\<rangle>,
-                           leq \<circ>\<^sub>c \<langle>right_cart_proj \<nat>\<^sub>c \<nat>\<^sub>c,left_cart_proj \<nat>\<^sub>c \<nat>\<^sub>c\<rangle>\<rangle>)\<^sup>\<sharp>) \<circ>\<^sub>c \<langle>n,m\<rangle>"
+          (OR \<circ>\<^sub>c \<langle>leq \<circ>\<^sub>c \<langle>left_cart_proj \<nat>\<^sub>c \<nat>\<^sub>c,right_cart_proj \<nat>\<^sub>c \<nat>\<^sub>c\<rangle>,
+                  leq \<circ>\<^sub>c \<langle>right_cart_proj \<nat>\<^sub>c \<nat>\<^sub>c,left_cart_proj \<nat>\<^sub>c \<nat>\<^sub>c\<rangle>\<rangle>)\<^sup>\<sharp> \<circ>\<^sub>c
+          successor) \<circ>\<^sub>c \<langle>n,m\<rangle> =
+         (eval_func \<Omega> \<nat>\<^sub>c \<circ>\<^sub>c id\<^sub>c \<nat>\<^sub>c \<times>\<^sub>f id\<^sub>c (\<Omega>\<^bsup>\<nat>\<^sub>c\<^esup>) \<circ>\<^sub>c
+          (OR \<circ>\<^sub>c \<langle>leq \<circ>\<^sub>c \<langle>left_cart_proj \<nat>\<^sub>c \<nat>\<^sub>c,right_cart_proj \<nat>\<^sub>c \<nat>\<^sub>c\<rangle>,
+                  leq \<circ>\<^sub>c \<langle>right_cart_proj \<nat>\<^sub>c \<nat>\<^sub>c,left_cart_proj \<nat>\<^sub>c \<nat>\<^sub>c\<rangle>\<rangle>)\<^sup>\<sharp>) \<circ>\<^sub>c \<langle>n,m\<rangle>"
               proof(cases "leq \<circ>\<^sub>c \<langle>n,m\<rangle> = \<f> \<and>  leq \<circ>\<^sub>c \<langle>m,n\<rangle> = \<f>", auto)  
                 assume "leq \<circ>\<^sub>c \<langle>n,m\<rangle> = \<f>"
                 assume "leq \<circ>\<^sub>c \<langle>m,n\<rangle> = \<f>"
+
                 have "(leq \<circ>\<^sub>c \<langle>n,successor \<circ>\<^sub>c m\<rangle> = \<f>)  \<and> (leq \<circ>\<^sub>c \<langle>successor \<circ>\<^sub>c m,n\<rangle> = \<f>)"
                  proof(rule ccontr,auto)
                    assume  "leq \<circ>\<^sub>c \<langle>n,successor \<circ>\<^sub>c m\<rangle> \<noteq> \<f>"
@@ -403,7 +486,8 @@ leq \<circ>\<^sub>c \<langle>right_cart_proj \<nat>\<^sub>c \<nat>\<^sub>c, left
                        using \<open>leq \<circ>\<^sub>c \<langle>m,n\<rangle> = \<f>\<close> \<open>leq \<circ>\<^sub>c \<langle>n,m\<rangle> = \<f>\<close> exists_implies_leq_true m_def by force
                    qed
                    then show False
-                     using \<open>leq \<circ>\<^sub>c \<langle>m,n\<rangle> = \<f>\<close> true_false_distinct by auto                 
+                     using \<open>leq \<circ>\<^sub>c \<langle>m,n\<rangle> = \<f>\<close> true_false_distinct by auto
+                 
                  next
                    assume "leq \<circ>\<^sub>c \<langle>successor \<circ>\<^sub>c m,n\<rangle> \<noteq> \<f>"
                    then have "leq \<circ>\<^sub>c \<langle>successor \<circ>\<^sub>c m,n\<rangle> = \<t>"
@@ -411,6 +495,7 @@ leq \<circ>\<^sub>c \<langle>right_cart_proj \<nat>\<^sub>c \<nat>\<^sub>c, left
                    then show False
                      by (metis \<open>leq \<circ>\<^sub>c \<langle>m,n\<rangle> = \<f>\<close>  add_respects_succ2 exists_implies_leq_true leq_true_implies_exists m_def succ_n_type true_false_distinct)
                  qed
+
               have "(eval_func \<Omega> \<nat>\<^sub>c \<circ>\<^sub>c id\<^sub>c \<nat>\<^sub>c \<times>\<^sub>f
           (OR \<circ>\<^sub>c \<langle>leq \<circ>\<^sub>c \<langle>left_cart_proj \<nat>\<^sub>c \<nat>\<^sub>c,right_cart_proj \<nat>\<^sub>c \<nat>\<^sub>c\<rangle>,
                   leq \<circ>\<^sub>c \<langle>right_cart_proj \<nat>\<^sub>c \<nat>\<^sub>c,left_cart_proj \<nat>\<^sub>c \<nat>\<^sub>c\<rangle>\<rangle>)\<^sup>\<sharp> \<circ>\<^sub>c
@@ -419,7 +504,10 @@ leq \<circ>\<^sub>c \<langle>right_cart_proj \<nat>\<^sub>c \<nat>\<^sub>c, left
                             (OR \<circ>\<^sub>c \<langle>leq \<circ>\<^sub>c \<langle>left_cart_proj \<nat>\<^sub>c \<nat>\<^sub>c,right_cart_proj \<nat>\<^sub>c \<nat>\<^sub>c\<rangle>,
                                     leq \<circ>\<^sub>c \<langle>right_cart_proj \<nat>\<^sub>c \<nat>\<^sub>c,left_cart_proj \<nat>\<^sub>c \<nat>\<^sub>c\<rangle>\<rangle>)\<^sup>\<sharp>) \<circ>\<^sub>c
                            (id\<^sub>c \<nat>\<^sub>c \<times>\<^sub>f successor) \<circ>\<^sub>c \<langle>n,m\<rangle>"
-                by (typecheck_cfuncs, smt cfunc_type_def comp_associative inv_transpose_func_def3 inv_transpose_of_composition m_def)
+                sorry
+(*
+                by (typecheck_cfuncs, smt cfunc_type_def comp_associative inv_transpose_func_def2 inv_transpose_of_composition m_def)
+*)
               also have "... = OR \<circ>\<^sub>c \<langle>leq \<circ>\<^sub>c \<langle>left_cart_proj \<nat>\<^sub>c \<nat>\<^sub>c,right_cart_proj \<nat>\<^sub>c \<nat>\<^sub>c\<rangle>,
                                     leq \<circ>\<^sub>c \<langle>right_cart_proj \<nat>\<^sub>c \<nat>\<^sub>c,left_cart_proj \<nat>\<^sub>c \<nat>\<^sub>c\<rangle>\<rangle>\<circ>\<^sub>c
                            (id\<^sub>c \<nat>\<^sub>c \<times>\<^sub>f successor) \<circ>\<^sub>c \<langle>n,m\<rangle>" 
@@ -439,6 +527,7 @@ leq \<circ>\<^sub>c \<langle>right_cart_proj \<nat>\<^sub>c \<nat>\<^sub>c, left
                 using left_cart_proj_cfunc_prod m_def right_cart_proj_cfunc_prod succ_n_type by auto     
               also have "... =  \<f>"
                 by (simp add: OR_false_false_is_false \<open>leq \<circ>\<^sub>c \<langle>n,successor \<circ>\<^sub>c m\<rangle> = \<f> \<and> leq \<circ>\<^sub>c \<langle>successor \<circ>\<^sub>c m,n\<rangle> = \<f>\<close>)
+
               have "(eval_func \<Omega> \<nat>\<^sub>c \<circ>\<^sub>c id\<^sub>c \<nat>\<^sub>c \<times>\<^sub>f id\<^sub>c (\<Omega>\<^bsup>\<nat>\<^sub>c\<^esup>) \<circ>\<^sub>c
           (OR \<circ>\<^sub>c \<langle>leq \<circ>\<^sub>c \<langle>left_cart_proj \<nat>\<^sub>c \<nat>\<^sub>c,right_cart_proj \<nat>\<^sub>c \<nat>\<^sub>c\<rangle>,
                   leq \<circ>\<^sub>c \<langle>right_cart_proj \<nat>\<^sub>c \<nat>\<^sub>c,left_cart_proj \<nat>\<^sub>c \<nat>\<^sub>c\<rangle>\<rangle>)\<^sup>\<sharp>) \<circ>\<^sub>c \<langle>n,m\<rangle> = \<f>"
@@ -449,7 +538,7 @@ leq \<circ>\<^sub>c \<langle>right_cart_proj \<nat>\<^sub>c \<nat>\<^sub>c, left
                     OR \<circ>\<^sub>c \<langle>leq \<circ>\<^sub>c \<langle>left_cart_proj \<nat>\<^sub>c \<nat>\<^sub>c,right_cart_proj \<nat>\<^sub>c \<nat>\<^sub>c\<rangle>,
                       leq \<circ>\<^sub>c \<langle>right_cart_proj \<nat>\<^sub>c \<nat>\<^sub>c,left_cart_proj \<nat>\<^sub>c \<nat>\<^sub>c\<rangle>\<rangle> \<circ>\<^sub>c \<langle>n,m\<rangle>"
                    by (typecheck_cfuncs, smt comp_associative2 id_left_unit2 m_def transpose_func_def x_is)
-                 also have "... = OR \<circ>\<^sub>c \<langle>leq \<circ>\<^sub>c \<langle>left_cart_proj \<nat>\<^sub>c \<nat>\<^sub>c \<circ>\<^sub>c \<langle>n,m\<rangle>  ,right_cart_proj \<nat>\<^sub>c \<nat>\<^sub>c \<circ>\<^sub>c \<langle>n,m\<rangle>\<rangle>,
+                 also have "... = OR \<circ>\<^sub>c \<langle>leq \<circ>\<^sub>c \<langle>left_cart_proj \<nat>\<^sub>c \<nat>\<^sub>c \<circ>\<^sub>c \<langle>n,m\<rangle>  ,right_cart_proj \<nat>\<^sub>c \<nat>\<^sub>c \<circ>\<^sub>c \<langle>n,m\<rangle> \<rangle>,
                     leq \<circ>\<^sub>c \<langle>right_cart_proj \<nat>\<^sub>c \<nat>\<^sub>c  \<circ>\<^sub>c \<langle>n,m\<rangle> ,left_cart_proj \<nat>\<^sub>c \<nat>\<^sub>c \<circ>\<^sub>c \<langle>n,m\<rangle> \<rangle>\<rangle> "
                    by (typecheck_cfuncs , smt cfunc_prod_comp comp_associative2 m_def x_is)
                  also have "... = OR \<circ>\<^sub>c \<langle>leq \<circ>\<^sub>c \<langle>n  ,m  \<rangle>, leq \<circ>\<^sub>c \<langle>m ,n \<rangle>\<rangle> "
@@ -459,14 +548,19 @@ leq \<circ>\<^sub>c \<langle>right_cart_proj \<nat>\<^sub>c \<nat>\<^sub>c, left
                  then show ?thesis
                    using calculation by auto
                qed
+
                then show ?thesis
-                 using \<open>OR \<circ>\<^sub>c \<langle>leq \<circ>\<^sub>c \<langle>n,successor \<circ>\<^sub>c m\<rangle>,leq \<circ>\<^sub>c \<langle>successor \<circ>\<^sub>c m,n\<rangle>\<rangle> = \<f>\<close> calculation by presburger              
+                 using \<open>OR \<circ>\<^sub>c \<langle>leq \<circ>\<^sub>c \<langle>n,successor \<circ>\<^sub>c m\<rangle>,leq \<circ>\<^sub>c \<langle>successor \<circ>\<^sub>c m,n\<rangle>\<rangle> = \<f>\<close> calculation by presburger
+              
               next
                 assume "leq \<circ>\<^sub>c \<langle>n,m\<rangle> \<noteq> \<f>"
                 then have "leq \<circ>\<^sub>c \<langle>n,m\<rangle> = \<t>"
                   using  m_def true_false_only_truth_values by (typecheck_cfuncs, blast)
+
                 then have "leq \<circ>\<^sub>c \<langle>n ,successor \<circ>\<^sub>c m\<rangle> = \<t>"
-                  by (metis add_respects_succ3 exists_implies_leq_true leq_true_implies_exists m_def succ_n_type)               
+                  by (metis add_respects_succ3 exists_implies_leq_true leq_true_implies_exists m_def succ_n_type)
+                
+                
                 have "(eval_func \<Omega> \<nat>\<^sub>c \<circ>\<^sub>c id\<^sub>c \<nat>\<^sub>c \<times>\<^sub>f
           (OR \<circ>\<^sub>c \<langle>leq \<circ>\<^sub>c \<langle>left_cart_proj \<nat>\<^sub>c \<nat>\<^sub>c,right_cart_proj \<nat>\<^sub>c \<nat>\<^sub>c\<rangle>,
                   leq \<circ>\<^sub>c \<langle>right_cart_proj \<nat>\<^sub>c \<nat>\<^sub>c,left_cart_proj \<nat>\<^sub>c \<nat>\<^sub>c\<rangle>\<rangle>)\<^sup>\<sharp> \<circ>\<^sub>c
@@ -475,7 +569,10 @@ leq \<circ>\<^sub>c \<langle>right_cart_proj \<nat>\<^sub>c \<nat>\<^sub>c, left
                             (OR \<circ>\<^sub>c \<langle>leq \<circ>\<^sub>c \<langle>left_cart_proj \<nat>\<^sub>c \<nat>\<^sub>c,right_cart_proj \<nat>\<^sub>c \<nat>\<^sub>c\<rangle>,
                                     leq \<circ>\<^sub>c \<langle>right_cart_proj \<nat>\<^sub>c \<nat>\<^sub>c,left_cart_proj \<nat>\<^sub>c \<nat>\<^sub>c\<rangle>\<rangle>)\<^sup>\<sharp>) \<circ>\<^sub>c
                            (id\<^sub>c \<nat>\<^sub>c \<times>\<^sub>f successor) \<circ>\<^sub>c \<langle>n,m\<rangle>"
-                by (typecheck_cfuncs, smt cfunc_type_def comp_associative inv_transpose_func_def3 inv_transpose_of_composition m_def)
+                  sorry
+                (*
+                by (typecheck_cfuncs, smt cfunc_type_def comp_associative inv_transpose_func_def2 inv_transpose_of_composition m_def)
+                *)
                 also have "... = OR \<circ>\<^sub>c \<langle>leq \<circ>\<^sub>c \<langle>left_cart_proj \<nat>\<^sub>c \<nat>\<^sub>c,right_cart_proj \<nat>\<^sub>c \<nat>\<^sub>c\<rangle>,
                                     leq \<circ>\<^sub>c \<langle>right_cart_proj \<nat>\<^sub>c \<nat>\<^sub>c,left_cart_proj \<nat>\<^sub>c \<nat>\<^sub>c\<rangle>\<rangle>\<circ>\<^sub>c
                            (id\<^sub>c \<nat>\<^sub>c \<times>\<^sub>f successor) \<circ>\<^sub>c \<langle>n,m\<rangle>" 
@@ -488,13 +585,14 @@ leq \<circ>\<^sub>c \<langle>right_cart_proj \<nat>\<^sub>c \<nat>\<^sub>c, left
                                     leq \<circ>\<^sub>c \<langle>right_cart_proj \<nat>\<^sub>c \<nat>\<^sub>c,left_cart_proj \<nat>\<^sub>c \<nat>\<^sub>c\<rangle>\<rangle>\<circ>\<^sub>c
                             \<langle>n,successor \<circ>\<^sub>c m\<rangle>"
                   using id_left_unit2 m_def by auto 
-                also have "... = OR \<circ>\<^sub>c \<langle>leq \<circ>\<^sub>c \<langle>left_cart_proj \<nat>\<^sub>c \<nat>\<^sub>c \<circ>\<^sub>c \<langle>n,successor \<circ>\<^sub>c m\<rangle>, right_cart_proj \<nat>\<^sub>c \<nat>\<^sub>c \<circ>\<^sub>c \<langle>n,successor \<circ>\<^sub>c m\<rangle>\<rangle>,
-                                    leq \<circ>\<^sub>c \<langle>right_cart_proj \<nat>\<^sub>c \<nat>\<^sub>c \<circ>\<^sub>c \<langle>n,successor \<circ>\<^sub>c m\<rangle>, left_cart_proj \<nat>\<^sub>c \<nat>\<^sub>c \<circ>\<^sub>c \<langle>n,successor \<circ>\<^sub>c m\<rangle>\<rangle>\<rangle>"
+                also have "... = OR \<circ>\<^sub>c \<langle>leq \<circ>\<^sub>c \<langle>left_cart_proj \<nat>\<^sub>c \<nat>\<^sub>c \<circ>\<^sub>c \<langle>n,successor \<circ>\<^sub>c m\<rangle> ,right_cart_proj \<nat>\<^sub>c \<nat>\<^sub>c \<circ>\<^sub>c \<langle>n,successor \<circ>\<^sub>c m\<rangle>\<rangle>  ,
+                                    leq \<circ>\<^sub>c \<langle>right_cart_proj \<nat>\<^sub>c \<nat>\<^sub>c \<circ>\<^sub>c \<langle>n,successor \<circ>\<^sub>c m\<rangle>   ,left_cart_proj \<nat>\<^sub>c \<nat>\<^sub>c \<circ>\<^sub>c \<langle>n,successor \<circ>\<^sub>c m\<rangle>  \<rangle>  \<rangle>"
                   using nsm_type by (typecheck_cfuncs, smt cfunc_prod_comp comp_associative2)
-               also have "... = OR \<circ>\<^sub>c \<langle>leq \<circ>\<^sub>c \<langle>n ,successor \<circ>\<^sub>c m\<rangle>,  leq \<circ>\<^sub>c \<langle>successor \<circ>\<^sub>c m, n\<rangle>\<rangle>"
+               also have "... = OR \<circ>\<^sub>c \<langle>leq \<circ>\<^sub>c \<langle>n ,successor \<circ>\<^sub>c m\<rangle>  ,  leq \<circ>\<^sub>c \<langle>successor \<circ>\<^sub>c m  ,n  \<rangle>\<rangle>"
                  using left_cart_proj_cfunc_prod m_def right_cart_proj_cfunc_prod succ_n_type by auto     
                also have "... =  \<t>"
                  using OR_true_left_is_true \<open>leq \<circ>\<^sub>c \<langle>n,successor \<circ>\<^sub>c m\<rangle> = \<t>\<close> comp_type leq_type smn_type by auto
+
               have "(eval_func \<Omega> \<nat>\<^sub>c \<circ>\<^sub>c id\<^sub>c \<nat>\<^sub>c \<times>\<^sub>f id\<^sub>c (\<Omega>\<^bsup>\<nat>\<^sub>c\<^esup>) \<circ>\<^sub>c
           (OR \<circ>\<^sub>c \<langle>leq \<circ>\<^sub>c \<langle>left_cart_proj \<nat>\<^sub>c \<nat>\<^sub>c,right_cart_proj \<nat>\<^sub>c \<nat>\<^sub>c\<rangle>,
                   leq \<circ>\<^sub>c \<langle>right_cart_proj \<nat>\<^sub>c \<nat>\<^sub>c,left_cart_proj \<nat>\<^sub>c \<nat>\<^sub>c\<rangle>\<rangle>)\<^sup>\<sharp>) \<circ>\<^sub>c \<langle>n,m\<rangle> = \<t>"
@@ -505,19 +603,22 @@ leq \<circ>\<^sub>c \<langle>right_cart_proj \<nat>\<^sub>c \<nat>\<^sub>c, left
                 OR \<circ>\<^sub>c \<langle>leq \<circ>\<^sub>c \<langle>left_cart_proj \<nat>\<^sub>c \<nat>\<^sub>c,right_cart_proj \<nat>\<^sub>c \<nat>\<^sub>c\<rangle>,
                   leq \<circ>\<^sub>c \<langle>right_cart_proj \<nat>\<^sub>c \<nat>\<^sub>c,left_cart_proj \<nat>\<^sub>c \<nat>\<^sub>c\<rangle>\<rangle> \<circ>\<^sub>c \<langle>n,m\<rangle>"
                  by (typecheck_cfuncs, smt comp_associative2 id_left_unit2 m_def transpose_func_def x_is)
-               also have "... = OR \<circ>\<^sub>c \<langle>leq \<circ>\<^sub>c \<langle>left_cart_proj \<nat>\<^sub>c \<nat>\<^sub>c \<circ>\<^sub>c \<langle>n,m\<rangle>  ,right_cart_proj \<nat>\<^sub>c \<nat>\<^sub>c \<circ>\<^sub>c \<langle>n,m\<rangle>\<rangle>,
-                  leq \<circ>\<^sub>c \<langle>right_cart_proj \<nat>\<^sub>c \<nat>\<^sub>c  \<circ>\<^sub>c \<langle>n,m\<rangle> ,left_cart_proj \<nat>\<^sub>c \<nat>\<^sub>c \<circ>\<^sub>c \<langle>n,m\<rangle>\<rangle>\<rangle> "
+               also have "... = OR \<circ>\<^sub>c \<langle>leq \<circ>\<^sub>c \<langle>left_cart_proj \<nat>\<^sub>c \<nat>\<^sub>c \<circ>\<^sub>c \<langle>n,m\<rangle>  ,right_cart_proj \<nat>\<^sub>c \<nat>\<^sub>c \<circ>\<^sub>c \<langle>n,m\<rangle> \<rangle>,
+                  leq \<circ>\<^sub>c \<langle>right_cart_proj \<nat>\<^sub>c \<nat>\<^sub>c  \<circ>\<^sub>c \<langle>n,m\<rangle> ,left_cart_proj \<nat>\<^sub>c \<nat>\<^sub>c \<circ>\<^sub>c \<langle>n,m\<rangle> \<rangle>\<rangle> "
                  by (typecheck_cfuncs , smt cfunc_prod_comp comp_associative2 m_def x_is)
-               also have "... = OR \<circ>\<^sub>c \<langle>leq \<circ>\<^sub>c \<langle>n,m\<rangle>, leq \<circ>\<^sub>c \<langle>m,n\<rangle>\<rangle> "
+               also have "... = OR \<circ>\<^sub>c \<langle>leq \<circ>\<^sub>c \<langle>n  ,m  \<rangle>, leq \<circ>\<^sub>c \<langle>m ,n \<rangle>\<rangle> "
                  by (typecheck_cfuncs, metis left_cart_proj_cfunc_prod m_def right_cart_proj_cfunc_prod)                             
                also have "... =  \<t>"
                  by (typecheck_cfuncs, simp add: OR_true_left_is_true \<open>leq \<circ>\<^sub>c \<langle>n,m\<rangle> = \<t>\<close> m_def)
+
                 then show ?thesis
-                  using calculation by auto
+                  by (simp add: \<open>(eval_func \<Omega> \<nat>\<^sub>c \<circ>\<^sub>c id\<^sub>c \<nat>\<^sub>c \<times>\<^sub>f id\<^sub>c (\<Omega>\<^bsup>\<nat>\<^sub>c\<^esup>) \<circ>\<^sub>c (OR \<circ>\<^sub>c \<langle>leq \<circ>\<^sub>c \<langle>left_cart_proj \<nat>\<^sub>c \<nat>\<^sub>c,right_cart_proj \<nat>\<^sub>c \<nat>\<^sub>c\<rangle>,leq \<circ>\<^sub>c \<langle>right_cart_proj \<nat>\<^sub>c \<nat>\<^sub>c,left_cart_proj \<nat>\<^sub>c \<nat>\<^sub>c\<rangle>\<rangle>)\<^sup>\<sharp>) \<circ>\<^sub>c \<langle>n,m\<rangle> = OR \<circ>\<^sub>c \<langle>leq \<circ>\<^sub>c \<langle>left_cart_proj \<nat>\<^sub>c \<nat>\<^sub>c,right_cart_proj \<nat>\<^sub>c \<nat>\<^sub>c\<rangle>,leq \<circ>\<^sub>c \<langle>right_cart_proj \<nat>\<^sub>c \<nat>\<^sub>c,left_cart_proj \<nat>\<^sub>c \<nat>\<^sub>c\<rangle>\<rangle> \<circ>\<^sub>c \<langle>n,m\<rangle>\<close> \<open>OR \<circ>\<^sub>c \<langle>leq \<circ>\<^sub>c \<langle>left_cart_proj \<nat>\<^sub>c \<nat>\<^sub>c \<circ>\<^sub>c \<langle>n,m\<rangle>,right_cart_proj \<nat>\<^sub>c \<nat>\<^sub>c \<circ>\<^sub>c \<langle>n,m\<rangle>\<rangle>,leq \<circ>\<^sub>c \<langle>right_cart_proj \<nat>\<^sub>c \<nat>\<^sub>c \<circ>\<^sub>c \<langle>n,m\<rangle>,left_cart_proj \<nat>\<^sub>c \<nat>\<^sub>c \<circ>\<^sub>c \<langle>n,m\<rangle>\<rangle>\<rangle> = OR \<circ>\<^sub>c \<langle>leq \<circ>\<^sub>c \<langle>n,m\<rangle>,leq \<circ>\<^sub>c \<langle>m,n\<rangle>\<rangle>\<close> \<open>OR \<circ>\<^sub>c \<langle>leq \<circ>\<^sub>c \<langle>left_cart_proj \<nat>\<^sub>c \<nat>\<^sub>c,right_cart_proj \<nat>\<^sub>c \<nat>\<^sub>c\<rangle>,leq \<circ>\<^sub>c \<langle>right_cart_proj \<nat>\<^sub>c \<nat>\<^sub>c,left_cart_proj \<nat>\<^sub>c \<nat>\<^sub>c\<rangle>\<rangle> \<circ>\<^sub>c \<langle>n,m\<rangle> = OR \<circ>\<^sub>c \<langle>leq \<circ>\<^sub>c \<langle>left_cart_proj \<nat>\<^sub>c \<nat>\<^sub>c \<circ>\<^sub>c \<langle>n,m\<rangle>,right_cart_proj \<nat>\<^sub>c \<nat>\<^sub>c \<circ>\<^sub>c \<langle>n,m\<rangle>\<rangle>,leq \<circ>\<^sub>c \<langle>right_cart_proj \<nat>\<^sub>c \<nat>\<^sub>c \<circ>\<^sub>c \<langle>n,m\<rangle>,left_cart_proj \<nat>\<^sub>c \<nat>\<^sub>c \<circ>\<^sub>c \<langle>n,m\<rangle>\<rangle>\<rangle>\<close> \<open>OR \<circ>\<^sub>c \<langle>leq \<circ>\<^sub>c \<langle>n,successor \<circ>\<^sub>c m\<rangle>,leq \<circ>\<^sub>c \<langle>successor \<circ>\<^sub>c m,n\<rangle>\<rangle> = \<t>\<close> calculation)
+
           next
               assume "leq \<circ>\<^sub>c \<langle>m,n\<rangle> \<noteq> \<f>"
               then have "leq \<circ>\<^sub>c \<langle>m,n\<rangle> = \<t>"
                 using  m_def true_false_only_truth_values by (typecheck_cfuncs, blast)
+
               then have "leq \<circ>\<^sub>c \<langle>m ,successor \<circ>\<^sub>c n\<rangle> = \<t>"
                 by (metis add_respects_succ3 exists_implies_leq_true leq_true_implies_exists m_def succ_n_type)                               
               have "(eval_func \<Omega> \<nat>\<^sub>c \<circ>\<^sub>c id\<^sub>c \<nat>\<^sub>c \<times>\<^sub>f
@@ -528,7 +629,10 @@ leq \<circ>\<^sub>c \<langle>right_cart_proj \<nat>\<^sub>c \<nat>\<^sub>c, left
                           (OR \<circ>\<^sub>c \<langle>leq \<circ>\<^sub>c \<langle>left_cart_proj \<nat>\<^sub>c \<nat>\<^sub>c,right_cart_proj \<nat>\<^sub>c \<nat>\<^sub>c\<rangle>,
                                   leq \<circ>\<^sub>c \<langle>right_cart_proj \<nat>\<^sub>c \<nat>\<^sub>c,left_cart_proj \<nat>\<^sub>c \<nat>\<^sub>c\<rangle>\<rangle>)\<^sup>\<sharp>) \<circ>\<^sub>c
                          (id\<^sub>c \<nat>\<^sub>c \<times>\<^sub>f successor) \<circ>\<^sub>c \<langle>n,m\<rangle>"
-                by (typecheck_cfuncs, smt cfunc_type_def comp_associative inv_transpose_func_def3 inv_transpose_of_composition m_def)
+                sorry
+                (*
+                by (typecheck_cfuncs, smt cfunc_type_def comp_associative inv_transpose_func_def2 inv_transpose_of_composition m_def)
+                *)
               also have "... = OR \<circ>\<^sub>c \<langle>leq \<circ>\<^sub>c \<langle>left_cart_proj \<nat>\<^sub>c \<nat>\<^sub>c,right_cart_proj \<nat>\<^sub>c \<nat>\<^sub>c\<rangle>,
                                   leq \<circ>\<^sub>c \<langle>right_cart_proj \<nat>\<^sub>c \<nat>\<^sub>c,left_cart_proj \<nat>\<^sub>c \<nat>\<^sub>c\<rangle>\<rangle>\<circ>\<^sub>c
                          (id\<^sub>c \<nat>\<^sub>c \<times>\<^sub>f successor) \<circ>\<^sub>c \<langle>n,m\<rangle>" 
@@ -548,6 +652,7 @@ leq \<circ>\<^sub>c \<langle>right_cart_proj \<nat>\<^sub>c \<nat>\<^sub>c, left
                using left_cart_proj_cfunc_prod m_def right_cart_proj_cfunc_prod succ_n_type by auto     
              also have "... =  \<t>"
                using OR_true_left_is_true \<open>leq \<circ>\<^sub>c \<langle>n,successor \<circ>\<^sub>c m\<rangle> = \<t>\<close> comp_type leq_type smn_type by auto
+
              have "(eval_func \<Omega> \<nat>\<^sub>c \<circ>\<^sub>c id\<^sub>c \<nat>\<^sub>c \<times>\<^sub>f id\<^sub>c (\<Omega>\<^bsup>\<nat>\<^sub>c\<^esup>) \<circ>\<^sub>c
         (OR \<circ>\<^sub>c \<langle>leq \<circ>\<^sub>c \<langle>left_cart_proj \<nat>\<^sub>c \<nat>\<^sub>c,right_cart_proj \<nat>\<^sub>c \<nat>\<^sub>c\<rangle>,
                 leq \<circ>\<^sub>c \<langle>right_cart_proj \<nat>\<^sub>c \<nat>\<^sub>c,left_cart_proj \<nat>\<^sub>c \<nat>\<^sub>c\<rangle>\<rangle>)\<^sup>\<sharp>) \<circ>\<^sub>c \<langle>n,m\<rangle> = \<t>"
@@ -599,6 +704,10 @@ leq \<circ>\<^sub>c \<langle>right_cart_proj \<nat>\<^sub>c \<nat>\<^sub>c, left
               then show ?thesis
                 using OR_true_right_is_true comp_type leq_type nsm_type by presburger
             qed
+            
+
+
+
 
             show "(eval_func \<Omega> \<nat>\<^sub>c \<circ>\<^sub>c id\<^sub>c \<nat>\<^sub>c \<times>\<^sub>f
                    (OR \<circ>\<^sub>c      \<langle>leq \<circ>\<^sub>c  \<langle>left_cart_proj \<nat>\<^sub>c  \<nat>\<^sub>c,right_cart_proj \<nat>\<^sub>c \<nat>\<^sub>c\<rangle>,
@@ -644,26 +753,29 @@ leq \<circ>\<^sub>c \<langle>right_cart_proj \<nat>\<^sub>c \<nat>\<^sub>c, left
                 using transpose_func_def by (typecheck_cfuncs, presburger)
               also have "... = (eval_func \<Omega> \<nat>\<^sub>c \<circ>\<^sub>c id\<^sub>c \<nat>\<^sub>c \<times>\<^sub>f id\<^sub>c (\<Omega>\<^bsup>\<nat>\<^sub>c\<^esup>) \<circ>\<^sub>c(OR \<circ>\<^sub>c \<langle>leq \<circ>\<^sub>c\<langle>left_cart_proj \<nat>\<^sub>c \<nat>\<^sub>c,right_cart_proj \<nat>\<^sub>c \<nat>\<^sub>c\<rangle>,
                                                                          leq \<circ>\<^sub>c \<langle>right_cart_proj \<nat>\<^sub>c \<nat>\<^sub>c,left_cart_proj \<nat>\<^sub>c \<nat>\<^sub>c\<rangle>\<rangle>)\<^sup>\<sharp>) \<circ>\<^sub>c \<langle>n,m\<rangle>"
-                by (typecheck_cfuncs, metis id_left_unit2)
-                then show ?thesis
+                using id_left_unit2 by (typecheck_cfuncs, auto)
+              then show ?thesis
                 by (simp add: calculation)
               qed
-          qed
-            then show "(eval_func \<Omega> \<nat>\<^sub>c \<circ>\<^sub>c id\<^sub>c \<nat>\<^sub>c \<times>\<^sub>f
+         qed
+
+              then show "(eval_func \<Omega> \<nat>\<^sub>c \<circ>\<^sub>c id\<^sub>c \<nat>\<^sub>c \<times>\<^sub>f
           (OR \<circ>\<^sub>c \<langle>leq \<circ>\<^sub>c \<langle>left_cart_proj \<nat>\<^sub>c \<nat>\<^sub>c,right_cart_proj \<nat>\<^sub>c \<nat>\<^sub>c\<rangle>,
                   leq \<circ>\<^sub>c \<langle>right_cart_proj \<nat>\<^sub>c \<nat>\<^sub>c,left_cart_proj \<nat>\<^sub>c \<nat>\<^sub>c\<rangle>\<rangle>)\<^sup>\<sharp> \<circ>\<^sub>c  successor) \<circ>\<^sub>c x =
          (eval_func \<Omega> \<nat>\<^sub>c \<circ>\<^sub>c id\<^sub>c \<nat>\<^sub>c \<times>\<^sub>f id\<^sub>c (\<Omega>\<^bsup>\<nat>\<^sub>c\<^esup>) \<circ>\<^sub>c
           (OR \<circ>\<^sub>c \<langle>leq \<circ>\<^sub>c \<langle>left_cart_proj \<nat>\<^sub>c \<nat>\<^sub>c,right_cart_proj \<nat>\<^sub>c \<nat>\<^sub>c\<rangle>,
                   leq \<circ>\<^sub>c \<langle>right_cart_proj \<nat>\<^sub>c \<nat>\<^sub>c,left_cart_proj \<nat>\<^sub>c \<nat>\<^sub>c\<rangle>\<rangle>)\<^sup>\<sharp>) \<circ>\<^sub>c x"
-            using  m_def by force           
+                using  m_def by force           
         qed
       qed
     qed
   qed
+
   have flat_main_result: "(OR \<circ>\<^sub>c \<langle>
                         leq \<circ>\<^sub>c \<langle>left_cart_proj \<nat>\<^sub>c \<nat>\<^sub>c, right_cart_proj \<nat>\<^sub>c \<nat>\<^sub>c\<rangle>,
                         leq \<circ>\<^sub>c \<langle>right_cart_proj \<nat>\<^sub>c \<nat>\<^sub>c, left_cart_proj \<nat>\<^sub>c \<nat>\<^sub>c\<rangle> \<rangle>) = \<t> \<circ>\<^sub>c \<beta>\<^bsub>\<nat>\<^sub>c\<times>\<^sub>c\<nat>\<^sub>c\<^esub>"
     by (typecheck_cfuncs, metis main_result transpose_func_def)
+
   have "(\<t> \<circ>\<^sub>c \<beta>\<^bsub>\<nat>\<^sub>c\<times>\<^sub>c\<nat>\<^sub>c\<^esub>) \<circ>\<^sub>c \<langle>m,n\<rangle> = \<t>"  
     using assms by (typecheck_cfuncs,  smt comp_associative2 id_right_unit2 id_type one_unique_element terminal_func_comp terminal_func_type)
   then  have calc1: "(OR \<circ>\<^sub>c \<langle>
@@ -688,8 +800,8 @@ qed
 lemma nat_strict_total_order:
   assumes "n \<in>\<^sub>c \<nat>\<^sub>c"
   assumes "m \<in>\<^sub>c \<nat>\<^sub>c"
-  shows "(n \<le>\<^sub>\<nat> m) = (\<not> successor \<circ>\<^sub>c m \<le>\<^sub>\<nat> n)"
-proof(safe)
+  shows "(n \<le>\<^sub>\<nat> m) = (\<not>(successor \<circ>\<^sub>c m \<le>\<^sub>\<nat> n))"
+proof(auto)
   show "n \<le>\<^sub>\<nat> m \<Longrightarrow> successor \<circ>\<^sub>c m \<le>\<^sub>\<nat> n \<Longrightarrow> False"
     by (metis add_respects_succ2 add_respects_zero_on_left exists_implies_leq_true leq_infix_def
         leq_transitivity lqe_antisymmetry n_neq_succ_n succ_n_type zero_type assms)
@@ -703,25 +815,31 @@ next
     using assms by (smt (verit, best) add_commutes add_respects_succ3 add_type exists_implies_leq_true leq_infix_def nonzero_is_succ succ_inject)
 qed
 
+
+
+
 lemma Succession_Principle:
   assumes n_type[type_rule]: "n \<in>\<^sub>c \<nat>\<^sub>c"
   shows "k \<in>\<^sub>c \<nat>\<^sub>c \<and>  n \<le>\<^sub>\<nat> k \<and> k \<le>\<^sub>\<nat> successor \<circ>\<^sub>c n \<Longrightarrow> k = n \<or> k = successor \<circ>\<^sub>c n"
-proof(unfold leq_infix_def, rule ccontr)
-  assume "k \<in>\<^sub>c \<nat>\<^sub>c \<and> leq \<circ>\<^sub>c \<langle>n,k\<rangle> = \<t> \<and> leq \<circ>\<^sub>c \<langle>k,successor \<circ>\<^sub>c n\<rangle> = \<t>"
-  then have k_type[type_rule]: "k \<in>\<^sub>c \<nat>\<^sub>c" and  n_lt_k: "leq \<circ>\<^sub>c \<langle>n,k\<rangle> = \<t>" and k_lt_sn: "leq \<circ>\<^sub>c \<langle>k,successor \<circ>\<^sub>c n\<rangle> = \<t>"
-    by (typecheck_cfuncs, linarith)
-  assume "\<not> (k = n \<or> k = successor \<circ>\<^sub>c n)"
-  then have k_not_n: "k \<noteq> n" and k_not_sn: "k \<noteq> successor \<circ>\<^sub>c n"
-      by (typecheck_cfuncs, linarith)
+proof(unfold leq_infix_def, rule ccontr, auto)
+  assume k_type[type_rule]: "k \<in>\<^sub>c \<nat>\<^sub>c"
+  assume k_not_n: "k \<noteq> n"
+  assume k_not_sn: "k \<noteq> successor \<circ>\<^sub>c n"
+  assume n_lt_k: "leq \<circ>\<^sub>c \<langle>n,k\<rangle> = \<t>"
+  assume k_lt_sn: "leq \<circ>\<^sub>c \<langle>k,successor \<circ>\<^sub>c n\<rangle> = \<t>"
+  
   obtain p where p_type[type_rule]: "p \<in>\<^sub>c \<nat>\<^sub>c" and p_def:  "k = p +\<^sub>\<nat> n" and p_nonzero: "p \<noteq> zero"
     by (typecheck_cfuncs, metis add_respects_zero_on_left k_not_n leq_true_implies_exists n_lt_k)
+
   obtain i where i_type[type_rule]: "i \<in>\<^sub>c \<nat>\<^sub>c" and i_def:  "p = successor \<circ>\<^sub>c i"
     using nonzero_is_succ p_nonzero by (typecheck_cfuncs, blast)
+
   obtain q where q_type[type_rule]: "q \<in>\<^sub>c \<nat>\<^sub>c" and q_def:  "successor \<circ>\<^sub>c n = q +\<^sub>\<nat> k"  and q_nonzero: "q \<noteq> zero"
     by (typecheck_cfuncs, metis add_respects_zero_on_left k_lt_sn k_not_sn leq_true_implies_exists)
+
   obtain j where j_type[type_rule]: "j \<in>\<^sub>c \<nat>\<^sub>c" and j_def:  "q = successor \<circ>\<^sub>c j"
     using nonzero_is_succ q_nonzero by (typecheck_cfuncs, blast)
-
+  
   have "successor \<circ>\<^sub>c k = successor \<circ>\<^sub>c (p +\<^sub>\<nat> n)"
     using p_def by blast
   then have "successor \<circ>\<^sub>c k = p +\<^sub>\<nat> (successor \<circ>\<^sub>c n)"
@@ -737,34 +855,107 @@ proof(unfold leq_infix_def, rule ccontr)
   then show False
     using add_type i_type j_type zero_is_not_successor by force
 qed
-  
+
+
+corollary lt_trichotomy:
+  assumes m_type: "m \<in>\<^sub>c \<nat>\<^sub>c" and n_type: "n \<in>\<^sub>c \<nat>\<^sub>c"
+  shows "m = n \<or> (m <\<^sub>\<nat> n) \<or> (n <\<^sub>\<nat> m)"
+proof -
+  have conn: "(leq \<circ>\<^sub>c \<langle>n, m\<rangle> = \<t>) \<or> (leq \<circ>\<^sub>c \<langle>m, n\<rangle> = \<t>)"
+    using lqe_connexity[OF m_type n_type] .
+
+  show ?thesis
+  proof (cases "leq \<circ>\<^sub>c \<langle>n, m\<rangle> = \<t>")
+    assume "leq \<circ>\<^sub>c \<langle>n, m\<rangle> = \<t>"
+    (* 1: n \<le> m *)
+    then have nm: "n \<le>\<^sub>\<nat> m"
+      by (simp add: leq_infix_def)
+
+
+    show ?thesis
+    proof (cases "m \<le>\<^sub>\<nat> n")
+      case True
+      (* m \<le> n and n \<le> m => m = n *)
+      then show ?thesis
+        by (simp add: \<open>leq \<circ>\<^sub>c \<langle>n,m\<rangle> = \<t>\<close> leq_infix_def lqe_antisymmetry m_type n_type)
+    next
+      assume "\<not> m \<le>\<^sub>\<nat> n"
+      (* \<not>(m \<le> n) => n < m by definition of < *)
+      then have "leq \<circ>\<^sub>c \<langle>m,n\<rangle> = \<f>"
+        using leq_infix_def m_type n_type true_false_only_truth_values by (typecheck_cfuncs, blast)
+      then have "NOT \<circ>\<^sub>c leq \<circ>\<^sub>c \<langle>m,n\<rangle> = \<t>"        
+        by (typecheck_cfuncs, simp add: NOT_false_is_true)
+      then have "n <\<^sub>\<nat> m"
+        by (typecheck_cfuncs, smt (verit, ccfv_threshold) NOT_type cfunc_prod_type comp_associative2
+            comp_type leq_type lt_def lt_infix_def m_type n_type swap_ap swap_def swap_type)
+      then show ?thesis by blast
+    qed
+  next
+    assume "leq \<circ>\<^sub>c \<langle>n,m\<rangle> \<noteq> \<t>"
+    (* 2: m \<le> n *)
+    then have mn: "m \<le>\<^sub>\<nat> n"
+      using conn leq_infix_def by blast
+
+    show ?thesis
+    proof (cases "n \<le>\<^sub>\<nat> m")
+      case True
+      (* n \<le> m and m \<le> n => m = n *)
+      have "m = n"
+        using True \<open>leq \<circ>\<^sub>c \<langle>n,m\<rangle> \<noteq> \<t>\<close> leq_infix_def by blast
+      then show ?thesis by blast
+    next
+      assume " \<not> n \<le>\<^sub>\<nat> m"
+   
+      (* \<not>(n \<le> m) => m < n *)
+      then have "leq \<circ>\<^sub>c \<langle>n,m\<rangle> = \<f>"
+        using leq_infix_def m_type n_type true_false_only_truth_values by (typecheck_cfuncs, blast)
+      then have "NOT \<circ>\<^sub>c leq \<circ>\<^sub>c \<langle>n,m\<rangle> = \<t>"        
+        by (typecheck_cfuncs, simp add: NOT_false_is_true)
+      then have "m <\<^sub>\<nat> n"
+        by (typecheck_cfuncs, smt (verit, ccfv_threshold) NOT_type cfunc_prod_type comp_associative2
+            comp_type leq_type lt_def lt_infix_def m_type n_type swap_ap swap_def swap_type)
+      then show ?thesis by blast
+    qed
+  qed
+qed
+
+(*We need to finish this proof! *)
+
 theorem strong_induction:
   assumes P_type[type_rule]: "P : \<nat>\<^sub>c \<rightarrow> \<Omega>" and n_type[type_rule]: "n \<in>\<^sub>c \<nat>\<^sub>c"
   assumes base_case: "P \<circ>\<^sub>c zero = \<t>"
   assumes induction_case: "\<And>n. n \<in>\<^sub>c \<nat>\<^sub>c \<Longrightarrow> (\<And>k. k \<in>\<^sub>c \<nat>\<^sub>c \<Longrightarrow> k \<le>\<^sub>\<nat> n \<Longrightarrow> P \<circ>\<^sub>c k = \<t>) \<Longrightarrow>   P \<circ>\<^sub>c (successor \<circ>\<^sub>c n) = \<t>"
   shows "P \<circ>\<^sub>c n = \<t>"
+  sorry
+
+
+(*
 proof - 
   obtain Q where Q_type[type_rule]: "Q : \<nat>\<^sub>c \<rightarrow> \<Omega>" 
-      and Q_def: "Q = FORALL \<nat>\<^sub>c  \<circ>\<^sub>c (IMPLIES \<circ>\<^sub>c \<langle>leq , P \<circ>\<^sub>c left_cart_proj \<nat>\<^sub>c \<nat>\<^sub>c\<rangle>)\<^sup>\<sharp>"
-    by (typecheck_cfuncs, blast)
-  have Qn_true_eqs: "\<And> n. n \<in>\<^sub>c \<nat>\<^sub>c \<Longrightarrow>(( Q \<circ>\<^sub>c n = \<t>) = (\<forall> k. k \<in>\<^sub>c \<nat>\<^sub>c \<longrightarrow> k \<le>\<^sub>\<nat> n \<longrightarrow> P \<circ>\<^sub>c k = \<t>))"
-  proof(safe)
+      and Q_def: "Q = (FORALL \<nat>\<^sub>c ) \<circ>\<^sub>c (IMPLIES \<circ>\<^sub>c \<langle>leq , P \<circ>\<^sub>c left_cart_proj \<nat>\<^sub>c \<nat>\<^sub>c\<rangle>)\<^sup>\<sharp>"
+    by typecheck_cfuncs
+  have "\<And> n. n \<in>\<^sub>c \<nat>\<^sub>c \<Longrightarrow>(( Q \<circ>\<^sub>c n = \<t>) = ( (\<forall> k. k \<in>\<^sub>c \<nat>\<^sub>c \<longrightarrow> k \<le>\<^sub>\<nat> n \<longrightarrow> P \<circ>\<^sub>c k = \<t>)))"
+  proof(auto)
     fix n 
     assume n_type[type_rule]: "n \<in>\<^sub>c \<nat>\<^sub>c"
     assume "Q \<circ>\<^sub>c n = \<t>"
-    then have "FORALL \<nat>\<^sub>c  \<circ>\<^sub>c (IMPLIES \<circ>\<^sub>c \<langle>leq , P \<circ>\<^sub>c left_cart_proj \<nat>\<^sub>c \<nat>\<^sub>c\<rangle>)\<^sup>\<sharp> \<circ>\<^sub>c n = \<t>"
+    then have "(FORALL \<nat>\<^sub>c ) \<circ>\<^sub>c (IMPLIES \<circ>\<^sub>c \<langle>leq , P \<circ>\<^sub>c left_cart_proj \<nat>\<^sub>c \<nat>\<^sub>c\<rangle>)\<^sup>\<sharp> \<circ>\<^sub>c n = \<t>"
       unfolding Q_def by (etcs_assocl, blast)
-    then have "FORALL \<nat>\<^sub>c  \<circ>\<^sub>c ((IMPLIES \<circ>\<^sub>c \<langle>leq , P \<circ>\<^sub>c left_cart_proj \<nat>\<^sub>c \<nat>\<^sub>c\<rangle>) \<circ>\<^sub>c (id  \<nat>\<^sub>c \<times>\<^sub>f n))\<^sup>\<sharp> = \<t>"
+    then have "(FORALL \<nat>\<^sub>c ) \<circ>\<^sub>c ((IMPLIES \<circ>\<^sub>c \<langle>leq , P \<circ>\<^sub>c left_cart_proj \<nat>\<^sub>c \<nat>\<^sub>c\<rangle> ) \<circ>\<^sub>c (id  \<nat>\<^sub>c \<times>\<^sub>f n)   )\<^sup>\<sharp> = \<t>"
       using  sharp_comp by (typecheck_cfuncs, force) 
-    then have "\<And>k.  k \<in>\<^sub>c \<nat>\<^sub>c \<Longrightarrow> (IMPLIES \<circ>\<^sub>c \<langle>leq , P \<circ>\<^sub>c left_cart_proj \<nat>\<^sub>c \<nat>\<^sub>c\<rangle>) \<circ>\<^sub>c( (id  \<nat>\<^sub>c \<times>\<^sub>f n) \<circ>\<^sub>c \<langle>k, id \<one>\<rangle>) = \<t>"
-      by(etcs_assocl, typecheck_cfuncs, smt FORALL_elim)
-    then have "\<And>k.  k \<in>\<^sub>c \<nat>\<^sub>c \<Longrightarrow> IMPLIES \<circ>\<^sub>c (\<langle>leq , P \<circ>\<^sub>c left_cart_proj \<nat>\<^sub>c \<nat>\<^sub>c\<rangle> \<circ>\<^sub>c \<langle>k,n\<rangle>) = \<t>"
-      by(etcs_assocl, typecheck_cfuncs, smt (z3)  cfunc_cross_prod_comp_cfunc_prod id_left_unit2 id_right_unit2 id_type)
-    then have "\<And>k.  k \<in>\<^sub>c \<nat>\<^sub>c \<Longrightarrow> IMPLIES \<circ>\<^sub>c (\<langle>leq \<circ>\<^sub>c \<langle>k, n\<rangle>, (P \<circ>\<^sub>c left_cart_proj \<nat>\<^sub>c \<nat>\<^sub>c) \<circ>\<^sub>c \<langle>k, n\<rangle>\<rangle>) = \<t>"
-      by (typecheck_cfuncs, smt (verit, ccfv_SIG) cfunc_prod_comp cfunc_prod_type)
-    then have "\<And>k.  k \<in>\<^sub>c \<nat>\<^sub>c \<Longrightarrow> IMPLIES \<circ>\<^sub>c (\<langle>leq \<circ>\<^sub>c \<langle>k, n\<rangle>, P \<circ>\<^sub>c k\<rangle>) = \<t>"
+    then have "\<And>k.  k \<in>\<^sub>c \<nat>\<^sub>c \<Longrightarrow> ((IMPLIES \<circ>\<^sub>c \<langle>leq , P \<circ>\<^sub>c left_cart_proj \<nat>\<^sub>c \<nat>\<^sub>c\<rangle> ) \<circ>\<^sub>c (id  \<nat>\<^sub>c \<times>\<^sub>f n)) \<circ>\<^sub>c \<langle>k   ,id \<one>  \<rangle>  = \<t> "
+      by (typecheck_cfuncs, meson FORALL_elim )
+    then have "\<And>k.  k \<in>\<^sub>c \<nat>\<^sub>c \<Longrightarrow> (IMPLIES \<circ>\<^sub>c \<langle>leq , P \<circ>\<^sub>c left_cart_proj \<nat>\<^sub>c \<nat>\<^sub>c\<rangle> ) \<circ>\<^sub>c( (id  \<nat>\<^sub>c \<times>\<^sub>f n) \<circ>\<^sub>c \<langle>k   ,id \<one>  \<rangle> ) = \<t> "
+      by(etcs_assocl, simp)
+    then have "\<And>k.  k \<in>\<^sub>c \<nat>\<^sub>c \<Longrightarrow> (IMPLIES \<circ>\<^sub>c \<langle>leq , P \<circ>\<^sub>c left_cart_proj \<nat>\<^sub>c \<nat>\<^sub>c\<rangle>) \<circ>\<^sub>c \<langle>k   ,n  \<rangle>  = \<t> "
+      by (typecheck_cfuncs, smt (z3)  cfunc_cross_prod_comp_cfunc_prod id_left_unit2 id_right_unit2 id_type)
+    then have "\<And>k.  k \<in>\<^sub>c \<nat>\<^sub>c \<Longrightarrow> IMPLIES \<circ>\<^sub>c (\<langle>leq , P \<circ>\<^sub>c left_cart_proj \<nat>\<^sub>c \<nat>\<^sub>c\<rangle> \<circ>\<^sub>c \<langle>k,n \<rangle>)  = \<t>"
+      by(etcs_assocl, simp)
+    then have "\<And>k.  k \<in>\<^sub>c \<nat>\<^sub>c \<Longrightarrow> IMPLIES \<circ>\<^sub>c (\<langle>leq \<circ>\<^sub>c \<langle>k, n\<rangle> , (P \<circ>\<^sub>c left_cart_proj \<nat>\<^sub>c \<nat>\<^sub>c) \<circ>\<^sub>c \<langle>k, n\<rangle>  \<rangle> )  = \<t>"
+      sorry
+    then have "\<And>k.  k \<in>\<^sub>c \<nat>\<^sub>c \<Longrightarrow> IMPLIES \<circ>\<^sub>c (\<langle>leq \<circ>\<^sub>c \<langle>k, n\<rangle> , P \<circ>\<^sub>c k  \<rangle> )  = \<t>"
       by (typecheck_cfuncs, metis cfunc_prod_type cfunc_type_def comp_associative left_cart_proj_cfunc_prod left_cart_proj_type)
-    then have "\<And>k.  k \<in>\<^sub>c \<nat>\<^sub>c \<Longrightarrow> leq \<circ>\<^sub>c \<langle>k, n\<rangle> = \<t> \<Longrightarrow> P \<circ>\<^sub>c k = \<t>"
+    then have "\<And>k.  k \<in>\<^sub>c \<nat>\<^sub>c \<Longrightarrow> leq \<circ>\<^sub>c \<langle>k, n\<rangle> = \<t> \<Longrightarrow> P \<circ>\<^sub>c k   = \<t>"
       by (typecheck_cfuncs, metis IMPLIES_elim' comp_type)
     then show "\<And> k.  k \<in>\<^sub>c \<nat>\<^sub>c \<Longrightarrow> k \<le>\<^sub>\<nat> n \<Longrightarrow> P \<circ>\<^sub>c k = \<t>"
       by(simp add: leq_infix_def)
@@ -772,37 +963,40 @@ proof -
     fix n 
     assume n_type[type_rule]: "n \<in>\<^sub>c \<nat>\<^sub>c"
     assume "\<forall>k. k \<in>\<^sub>c \<nat>\<^sub>c \<longrightarrow> k \<le>\<^sub>\<nat> n \<longrightarrow> P \<circ>\<^sub>c k = \<t>"
-    then have "\<And> k.  k \<in>\<^sub>c \<nat>\<^sub>c \<Longrightarrow> leq \<circ>\<^sub>c \<langle>k, n\<rangle> = \<t> \<Longrightarrow> P \<circ>\<^sub>c k = \<t>"
+    then have "\<And> k.  k \<in>\<^sub>c \<nat>\<^sub>c \<Longrightarrow> leq \<circ>\<^sub>c \<langle>k, n\<rangle> = \<t> \<Longrightarrow> P \<circ>\<^sub>c k   = \<t>"
       using leq_infix_def by blast
-    then have "\<And>k.  k \<in>\<^sub>c \<nat>\<^sub>c \<Longrightarrow> IMPLIES \<circ>\<^sub>c (\<langle>leq \<circ>\<^sub>c \<langle>k, n\<rangle>, P \<circ>\<^sub>c k\<rangle>) = \<t>"
+    then have "\<And>k.  k \<in>\<^sub>c \<nat>\<^sub>c \<Longrightarrow> IMPLIES \<circ>\<^sub>c (\<langle>leq \<circ>\<^sub>c \<langle>k, n\<rangle> , P \<circ>\<^sub>c k  \<rangle> )  = \<t>"
       by (typecheck_cfuncs, smt (verit, ccfv_SIG)  cfunc_prod_type comp_type implies_implies_IMPLIES)
-    then have "\<And>k.  k \<in>\<^sub>c \<nat>\<^sub>c \<Longrightarrow> IMPLIES \<circ>\<^sub>c (\<langle>leq \<circ>\<^sub>c \<langle>k, n\<rangle>, (P \<circ>\<^sub>c left_cart_proj \<nat>\<^sub>c \<nat>\<^sub>c) \<circ>\<^sub>c \<langle>k, n\<rangle>\<rangle>) = \<t>"
-      by(etcs_assocr, typecheck_cfuncs, simp add:  left_cart_proj_cfunc_prod)
-    then have "\<And>k.  k \<in>\<^sub>c \<nat>\<^sub>c \<Longrightarrow> (IMPLIES \<circ>\<^sub>c \<langle>leq, P \<circ>\<^sub>c left_cart_proj \<nat>\<^sub>c \<nat>\<^sub>c\<rangle>) \<circ>\<^sub>c \<langle>k, n\<rangle> = \<t>"
-      by (etcs_assocr, typecheck_cfuncs, smt (verit, best) cfunc_prod_comp cfunc_prod_type)
-    then have "\<And>k.  k \<in>\<^sub>c \<nat>\<^sub>c \<Longrightarrow> ((IMPLIES \<circ>\<^sub>c \<langle>leq, P \<circ>\<^sub>c left_cart_proj \<nat>\<^sub>c \<nat>\<^sub>c\<rangle>) \<circ>\<^sub>c (id  \<nat>\<^sub>c \<times>\<^sub>f n)) \<circ>\<^sub>c \<langle>k   ,id \<one>  \<rangle> = \<t>"
-      by (typecheck_cfuncs, smt (verit, best)  cfunc_cross_prod_comp_cfunc_prod cfunc_prod_type comp_associative2 id_left_unit2 id_right_unit2)
-    then have "FORALL \<nat>\<^sub>c  \<circ>\<^sub>c ((IMPLIES \<circ>\<^sub>c \<langle>leq, P \<circ>\<^sub>c left_cart_proj \<nat>\<^sub>c \<nat>\<^sub>c\<rangle>) \<circ>\<^sub>c (id  \<nat>\<^sub>c \<times>\<^sub>f n))\<^sup>\<sharp> = \<t>"
-      using all_true_implies_FORALL_true3 by (typecheck_cfuncs, blast)
-    then have "FORALL \<nat>\<^sub>c  \<circ>\<^sub>c (IMPLIES \<circ>\<^sub>c \<langle>leq, P \<circ>\<^sub>c left_cart_proj \<nat>\<^sub>c \<nat>\<^sub>c\<rangle>)\<^sup>\<sharp> \<circ>\<^sub>c n = \<t>"
-      by (typecheck_cfuncs, simp add: sharp_comp)
-    then show "Q \<circ>\<^sub>c n = \<t>"
-      unfolding Q_def by (etcs_assocr, blast)
-  qed
+    then have "\<And>k.  k \<in>\<^sub>c \<nat>\<^sub>c \<Longrightarrow> IMPLIES \<circ>\<^sub>c (\<langle>leq \<circ>\<^sub>c \<langle>k, n\<rangle> , P \<circ>\<^sub>c (left_cart_proj \<nat>\<^sub>c \<nat>\<^sub>c \<circ>\<^sub>c \<langle>k, n\<rangle>)  \<rangle> )  = \<t>"
+      by (typecheck_cfuncs, simp add:  left_cart_proj_cfunc_prod) 
+    then have "\<And>k.  k \<in>\<^sub>c \<nat>\<^sub>c \<Longrightarrow> IMPLIES \<circ>\<^sub>c (\<langle>leq \<circ>\<^sub>c \<langle>k, n\<rangle> , (P \<circ>\<^sub>c left_cart_proj \<nat>\<^sub>c \<nat>\<^sub>c) \<circ>\<^sub>c \<langle>k, n\<rangle>  \<rangle> )  = \<t>"
+      by(etcs_assocr, simp)
+    then have "\<And>k.  k \<in>\<^sub>c \<nat>\<^sub>c \<Longrightarrow> IMPLIES \<circ>\<^sub>c (\<langle>leq , P \<circ>\<^sub>c left_cart_proj \<nat>\<^sub>c \<nat>\<^sub>c\<rangle> \<circ>\<^sub>c \<langle>k,n \<rangle>)  = \<t>"
+      oops
+*)
+
+
+
+
+
+(*    
   have "Q \<circ>\<^sub>c n = \<t>"
   proof(etcs_rule nat_induction)
     show "Q \<circ>\<^sub>c zero = \<t>"
-      using Q_def Qn_true_eqs base_case leq_infix_def lqe_antisymmetry true_false_distinct zero_is_smallest by (typecheck_cfuncs, blast)
-  next
-    fix n 
-    assume n_type[type_rule]: "n \<in>\<^sub>c \<nat>\<^sub>c"
-    assume Qn_true:  "Q \<circ>\<^sub>c n = \<t>"
-    then show "Q \<circ>\<^sub>c successor \<circ>\<^sub>c n = \<t>"
-       by (typecheck_cfuncs, metis Qn_true_eqs induction_case leq_infix_def lqe_antisymmetry nat_strict_total_order)
-  qed
-  then show "P \<circ>\<^sub>c n = \<t>"
-    using Qn_true_eqs leq_infix_def lqe_connexity by (typecheck_cfuncs, blast)
-qed
+        proof - 
+          fix n 
+          assume n_type[type_rule]: "n \<in>\<^sub>c \<nat>\<^sub>c"
+          *)
+ 
+  
+  
+  
+
+
+
+
+
+
 
 theorem well_ordering_principle:
   assumes nonempty_set: "nonempty S"  
@@ -810,10 +1004,10 @@ theorem well_ordering_principle:
   shows "\<exists> min. min \<in>\<^bsub>\<nat>\<^sub>c\<^esub> (S, m) \<and> (\<forall> s. s \<in>\<^bsub>\<nat>\<^sub>c\<^esub> (S, m) \<longrightarrow> min  \<le>\<^sub>\<nat> s)"
 proof(rule ccontr) 
   assume no_min: "\<nexists>min. min \<in>\<^bsub>\<nat>\<^sub>c\<^esub> (S, m) \<and> (\<forall>s. s \<in>\<^bsub>\<nat>\<^sub>c\<^esub> (S, m) \<longrightarrow> min \<le>\<^sub>\<nat> s)"
-  obtain P where P_type[type_rule]: "P : \<nat>\<^sub>c \<rightarrow> \<Omega>" and P_def: "P = NOT \<circ>\<^sub>c characteristic_func m"
+  obtain P where P_type[type_rule]: "P : \<nat>\<^sub>c \<rightarrow> \<Omega>" and P_def: "P = NOT \<circ>\<^sub>c (characteristic_func m)"
     by (metis NOT_type characteristic_func_type comp_type subobject_of_def2 subset_nat)
   have P_eq_t: "\<And> n. n \<in>\<^sub>c \<nat>\<^sub>c \<longrightarrow> P \<circ>\<^sub>c n  = \<t>"
-  proof(clarify)
+  proof(auto)
     fix n 
     assume n_type[type_rule]: "n \<in>\<^sub>c \<nat>\<^sub>c"
     show "P \<circ>\<^sub>c n  = \<t>"
@@ -821,9 +1015,14 @@ proof(rule ccontr)
       show "P \<circ>\<^sub>c zero = \<t>"
       proof(rule ccontr)
         assume "P \<circ>\<^sub>c zero \<noteq> \<t>"
-        then have "zero \<in>\<^bsub>\<nat>\<^sub>c\<^esub> (S, m)"
-          by (typecheck_cfuncs, metis NOT_false_is_true NOT_type P_def  characteristic_func_type comp_associative2 not_rel_mem_char_func_false subobject_of_def2 subset_nat)
-        have "\<forall> s. s \<in>\<^bsub>\<nat>\<^sub>c\<^esub> (S, m) \<longrightarrow>  zero \<le>\<^sub>\<nat>  s"
+        then have "P \<circ>\<^sub>c zero = \<f>"
+          by (typecheck_cfuncs, metis true_false_only_truth_values)
+        have "zero \<in>\<^bsub>\<nat>\<^sub>c\<^esub> (S, m)"
+          by (metis NOT_false_is_true NOT_type P_def \<open>P \<circ>\<^sub>c zero \<noteq> \<t>\<close> 
+              characteristic_func_type comp_associative2 not_rel_mem_char_func_false 
+              subobject_of_def2 subset_nat zero_type)
+          
+        have "(\<forall> s. s \<in>\<^bsub>\<nat>\<^sub>c\<^esub> (S, m) \<longrightarrow>  zero \<le>\<^sub>\<nat>  s)"
           by (simp add: leq_infix_def relative_member_def zero_is_smallest)
         then show False
           using no_min \<open>zero \<in>\<^bsub>\<nat>\<^sub>c\<^esub> (S, m)\<close> by blast
@@ -833,34 +1032,38 @@ proof(rule ccontr)
         fix n 
         assume n_type[type_rule]: "n \<in>\<^sub>c \<nat>\<^sub>c"
         assume "(\<And>k. k \<in>\<^sub>c \<nat>\<^sub>c \<Longrightarrow> k \<le>\<^sub>\<nat> n \<Longrightarrow> P \<circ>\<^sub>c k = \<t>)"
-        then have induction_hypothesis: "\<And>k. k \<in>\<^sub>c \<nat>\<^sub>c \<Longrightarrow> k \<le>\<^sub>\<nat> n \<Longrightarrow> \<not>k \<in>\<^bsub>\<nat>\<^sub>c\<^esub> (S, m)"
-          by (metis NOT_true_is_false NOT_type P_def  characteristic_func_false_not_relative_member
-              characteristic_func_type comp_associative2 rel_mem_char_func_true subobject_of_def2 subset_nat)
-        have "\<not>successor \<circ>\<^sub>c n  \<in>\<^bsub>\<nat>\<^sub>c\<^esub> (S, m)"
-        proof(rule ccontr, clarify)
+        then have induction_hypothesis: "(\<And>k. k \<in>\<^sub>c \<nat>\<^sub>c \<Longrightarrow> k \<le>\<^sub>\<nat> n \<Longrightarrow> \<not>(k \<in>\<^bsub>\<nat>\<^sub>c\<^esub> (S, m)))"
+          by (typecheck_cfuncs, metis NOT_true_is_false NOT_type P_def 
+              \<open>\<And>k. k \<in>\<^sub>c \<nat>\<^sub>c \<Longrightarrow> k \<le>\<^sub>\<nat> n \<Longrightarrow> P \<circ>\<^sub>c k = \<t>\<close> cfunc_type_def characteristic_func_type 
+              comp_associative rel_mem_char_func_true relative_member_def2 true_false_distinct)
+        have "\<not>(successor \<circ>\<^sub>c n  \<in>\<^bsub>\<nat>\<^sub>c\<^esub> (S, m))"
+        proof(rule ccontr, auto)
           assume BWOC: "successor \<circ>\<^sub>c n  \<in>\<^bsub>\<nat>\<^sub>c\<^esub> (S, m)"
-          then have "\<forall> s. s \<in>\<^bsub>\<nat>\<^sub>c\<^esub> (S, m) \<longrightarrow> successor \<circ>\<^sub>c n  \<le>\<^sub>\<nat> s "
+          then have "(\<forall> s. s \<in>\<^bsub>\<nat>\<^sub>c\<^esub> (S, m) \<longrightarrow> successor \<circ>\<^sub>c n  \<le>\<^sub>\<nat> s )"
             by (typecheck_cfuncs, metis Succession_Principle induction_hypothesis leq_infix_def lqe_connexity relative_member_def2)
           then show False
             using BWOC no_min by blast
         qed
         then show "P \<circ>\<^sub>c successor \<circ>\<^sub>c n = \<t>"
+          sorry
+(*
           by (typecheck_cfuncs, metis NOT_false_is_true NOT_type P_def  characteristic_func_type 
-              comp_associative2 not_rel_mem_char_func_false subobject_of_def2 subset_nat)
+              comp_associative2 rel_mem_char_func_true subobject_of_def2 subset_nat)
+*)
       qed
     qed
   qed
-  have "\<not> nonempty S"
-  proof(rule ccontr, clarify, unfold nonempty_def)
+  have "\<not>(nonempty S)"
+  proof(rule ccontr, auto, unfold nonempty_def)
     assume "\<exists>s. s \<in>\<^sub>c S"
     then obtain s where s_type[type_rule]: "s \<in>\<^sub>c S"
       by blast
-    then have "P \<circ>\<^sub>c m  \<circ>\<^sub>c s = \<t>"
+    then have "P \<circ>\<^sub>c (m  \<circ>\<^sub>c s) = \<t>"
       using P_eq_t comp_type subobject_of_def2 subset_nat by blast
-    then have "\<not> m  \<circ>\<^sub>c s  \<in>\<^bsub>\<nat>\<^sub>c\<^esub> (S, m)"
+    then have "\<not> (m  \<circ>\<^sub>c s  \<in>\<^bsub>\<nat>\<^sub>c\<^esub> (S, m))"
       by (metis NOT_true_is_false NOT_type P_def characteristic_func_type comp_associative2
           rel_mem_char_func_true relative_member_def2 true_false_distinct)
-    then have "\<nexists>h. m \<circ>\<^sub>c h = m \<circ>\<^sub>c s"
+    then have "\<nexists>h. (m \<circ>\<^sub>c h = m \<circ>\<^sub>c s)"
       by (typecheck_cfuncs, meson factors_through_def2 relative_member_def2 subobject_of_def2 subset_nat)
     then show False
       by blast
@@ -868,5 +1071,9 @@ proof(rule ccontr)
   then show False
     using nonempty_set by auto
 qed
+
+
+
+
 
 end
