Primitive_Recursive.thy
@@ -1,5 +1,5 @@
-theory Primitive_Recursive
-  imports Category_Set.ETCS
+theory Primitive_Recursive 
+  imports "Category_Set_Arithmetic/Inequality"
 begin
 
 theorem nat_eq_induction:
@@ -28,9 +28,8 @@ proof -
   then show "f \<circ>\<^sub>c n = g \<circ>\<^sub>c n"
     by (typecheck_cfuncs_prems, smt cfunc_prod_comp comp_associative2 comp_type eq_pred_iff_eq)
 qed
-      
-
-lemma primitive_recursion:
+     
+theorem primitive_recursion:
   assumes f0_type[type_rule]: "f0 : A \<rightarrow> B"
   assumes f_type[type_rule]: "f : A \<times>\<^sub>c (\<nat>\<^sub>c \<times>\<^sub>c B) \<rightarrow> B"
   shows "\<exists>!u. u : A \<times>\<^sub>c \<nat>\<^sub>c \<rightarrow> B \<and> (\<forall> a n. (a \<in>\<^sub>c A \<and> n \<in>\<^sub>c \<nat>\<^sub>c) \<longrightarrow>
@@ -55,14 +54,14 @@ proof -
     assume a_type[type_rule]: "a \<in>\<^sub>c A"
 
     show "(left_cart_proj \<nat>\<^sub>c B \<circ>\<^sub>c y\<^sup>\<flat> \<circ>\<^sub>c \<langle>a \<circ>\<^sub>c \<beta>\<^bsub>\<nat>\<^sub>c\<^esub>,id\<^sub>c \<nat>\<^sub>c\<rangle>) \<circ>\<^sub>c zero = id\<^sub>c \<nat>\<^sub>c \<circ>\<^sub>c zero"
-    proof - 
+    proof -
       have "(left_cart_proj \<nat>\<^sub>c B \<circ>\<^sub>c y\<^sup>\<flat> \<circ>\<^sub>c \<langle>a \<circ>\<^sub>c \<beta>\<^bsub>\<nat>\<^sub>c\<^esub>,id\<^sub>c \<nat>\<^sub>c\<rangle>) \<circ>\<^sub>c zero = left_cart_proj \<nat>\<^sub>c B \<circ>\<^sub>c y\<^sup>\<flat> \<circ>\<^sub>c \<langle>a \<circ>\<^sub>c \<beta>\<^bsub>\<nat>\<^sub>c\<^esub> \<circ>\<^sub>c zero,id\<^sub>c \<nat>\<^sub>c \<circ>\<^sub>c zero\<rangle>"
         by (etcs_assocr, typecheck_cfuncs, simp add: cfunc_prod_comp comp_associative2)
       also have "... = left_cart_proj \<nat>\<^sub>c B \<circ>\<^sub>c y\<^sup>\<flat> \<circ>\<^sub>c \<langle>a, zero\<rangle>"
         by (typecheck_cfuncs, metis id_left_unit2 id_right_unit2 id_type one_unique_element)
       also have "... = left_cart_proj \<nat>\<^sub>c B \<circ>\<^sub>c (y\<^sup>\<flat> \<circ>\<^sub>c (id A \<times>\<^sub>f zero)) \<circ>\<^sub>c \<langle>a, id \<one>\<rangle>"
         by (etcs_assocr, typecheck_cfuncs, simp add: cfunc_cross_prod_comp_cfunc_prod id_left_unit2 id_right_unit2)
-      also have "... = left_cart_proj \<nat>\<^sub>c B \<circ>\<^sub>c \<langle>zero \<circ>\<^sub>c \<beta>\<^bsub>A \<times>\<^sub>c \<one>\<^esub> \<circ>\<^sub>c \<langle>a, id \<one>\<rangle>,  f0 \<circ>\<^sub>c left_cart_proj A \<one> \<circ>\<^sub>c \<langle>a, id \<one>\<rangle>\<rangle>" 
+      also have "... = left_cart_proj \<nat>\<^sub>c B \<circ>\<^sub>c \<langle>zero \<circ>\<^sub>c \<beta>\<^bsub>A \<times>\<^sub>c \<one>\<^esub> \<circ>\<^sub>c \<langle>a, id \<one>\<rangle>,  f0 \<circ>\<^sub>c left_cart_proj A \<one> \<circ>\<^sub>c \<langle>a, id \<one>\<rangle>\<rangle>"
         by (etcs_assocl, typecheck_cfuncs, smt (verit, best) comp_associative2 left_cart_proj_cfunc_prod yb_zero)
       also have "... = zero \<circ>\<^sub>c \<beta>\<^bsub>A \<times>\<^sub>c \<one>\<^esub> \<circ>\<^sub>c \<langle>a, id \<one>\<rangle>"
         using left_cart_proj_cfunc_prod by (typecheck_cfuncs, simp)
@@ -70,12 +69,12 @@ proof -
         by (typecheck_cfuncs, metis id_left_unit2 id_right_unit2 one_unique_element)
       finally show ?thesis.
     qed
-      
+     
 
     show "(left_cart_proj \<nat>\<^sub>c B \<circ>\<^sub>c y\<^sup>\<flat> \<circ>\<^sub>c \<langle>a \<circ>\<^sub>c \<beta>\<^bsub>\<nat>\<^sub>c\<^esub>,id\<^sub>c \<nat>\<^sub>c\<rangle>) \<circ>\<^sub>c successor =
          successor \<circ>\<^sub>c left_cart_proj \<nat>\<^sub>c B \<circ>\<^sub>c y\<^sup>\<flat> \<circ>\<^sub>c \<langle>a \<circ>\<^sub>c \<beta>\<^bsub>\<nat>\<^sub>c\<^esub>,id\<^sub>c \<nat>\<^sub>c\<rangle>"
     proof -
-      have "(left_cart_proj \<nat>\<^sub>c B \<circ>\<^sub>c y\<^sup>\<flat> \<circ>\<^sub>c \<langle>a \<circ>\<^sub>c \<beta>\<^bsub>\<nat>\<^sub>c\<^esub>,id\<^sub>c \<nat>\<^sub>c\<rangle>) \<circ>\<^sub>c  successor = 
+      have "(left_cart_proj \<nat>\<^sub>c B \<circ>\<^sub>c y\<^sup>\<flat> \<circ>\<^sub>c \<langle>a \<circ>\<^sub>c \<beta>\<^bsub>\<nat>\<^sub>c\<^esub>,id\<^sub>c \<nat>\<^sub>c\<rangle>) \<circ>\<^sub>c  successor =
                  left_cart_proj \<nat>\<^sub>c B \<circ>\<^sub>c y\<^sup>\<flat> \<circ>\<^sub>c \<langle>a \<circ>\<^sub>c \<beta>\<^bsub>\<nat>\<^sub>c\<^esub>, successor\<rangle>"
         by (typecheck_cfuncs, smt cfunc_prod_comp comp_associative2 id_left_unit2 terminal_func_comp)
       also have "... = left_cart_proj \<nat>\<^sub>c B \<circ>\<^sub>c (y\<^sup>\<flat> \<circ>\<^sub>c (id A \<times>\<^sub>f successor)) \<circ>\<^sub>c \<langle>a \<circ>\<^sub>c \<beta>\<^bsub>\<nat>\<^sub>c\<^esub>,id\<^sub>c \<nat>\<^sub>c\<rangle>"
@@ -86,7 +85,7 @@ proof -
         using comp_associative2 left_cart_proj_cfunc_prod by (typecheck_cfuncs, auto)
       also have "... = successor \<circ>\<^sub>c left_cart_proj \<nat>\<^sub>c B \<circ>\<^sub>c  eval_func (\<nat>\<^sub>c \<times>\<^sub>c B) A \<circ>\<^sub>c (id A \<times>\<^sub>f y) \<circ>\<^sub>c \<langle>a \<circ>\<^sub>c \<beta>\<^bsub>\<nat>\<^sub>c\<^esub>,id\<^sub>c \<nat>\<^sub>c\<rangle>"
         by (typecheck_cfuncs, smt (verit, ccfv_threshold) comp_associative2 right_cart_proj_cfunc_prod)
-      also have "... = successor \<circ>\<^sub>c left_cart_proj \<nat>\<^sub>c B \<circ>\<^sub>c y\<^sup>\<flat> \<circ>\<^sub>c \<langle>a \<circ>\<^sub>c \<beta>\<^bsub>\<nat>\<^sub>c\<^esub>,id\<^sub>c \<nat>\<^sub>c\<rangle>"           
+      also have "... = successor \<circ>\<^sub>c left_cart_proj \<nat>\<^sub>c B \<circ>\<^sub>c y\<^sup>\<flat> \<circ>\<^sub>c \<langle>a \<circ>\<^sub>c \<beta>\<^bsub>\<nat>\<^sub>c\<^esub>,id\<^sub>c \<nat>\<^sub>c\<rangle>"          
         by (typecheck_cfuncs, smt (verit, best) cfunc_cross_prod_comp_cfunc_prod comp_associative2 id_left_unit2 id_right_unit2 inv_transpose_func_def3)
       finally show ?thesis .
     qed
@@ -100,7 +99,7 @@ proof -
     show "right_cart_proj \<nat>\<^sub>c B \<circ>\<^sub>c y\<^sup>\<flat> : A \<times>\<^sub>c \<nat>\<^sub>c \<rightarrow> B"
       by typecheck_cfuncs
     show g1: "\<And>a n. a \<in>\<^sub>c A \<Longrightarrow> n \<in>\<^sub>c \<nat>\<^sub>c \<Longrightarrow> (right_cart_proj \<nat>\<^sub>c B \<circ>\<^sub>c y\<^sup>\<flat>) \<circ>\<^sub>c \<langle>a,zero\<rangle> = f0 \<circ>\<^sub>c a"
-    proof - 
+    proof -
       fix a n
       assume a_type[type_rule]: "a \<in>\<^sub>c A"
       assume n_type[type_rule]: "n \<in>\<^sub>c \<nat>\<^sub>c"
@@ -118,7 +117,7 @@ proof -
       qed
     qed
     show g2: "\<And>a n. a \<in>\<^sub>c A \<Longrightarrow> n \<in>\<^sub>c \<nat>\<^sub>c \<Longrightarrow> (right_cart_proj \<nat>\<^sub>c B \<circ>\<^sub>c y\<^sup>\<flat>) \<circ>\<^sub>c \<langle>a,successor \<circ>\<^sub>c n\<rangle> = f \<circ>\<^sub>c \<langle>a,\<langle>n,(right_cart_proj \<nat>\<^sub>c B \<circ>\<^sub>c y\<^sup>\<flat>) \<circ>\<^sub>c \<langle>a,n\<rangle>\<rangle>\<rangle>"
-    proof - 
+    proof -
       fix a n
       assume a_type[type_rule]: "a \<in>\<^sub>c A"
       assume n_type[type_rule]: "n \<in>\<^sub>c \<nat>\<^sub>c"
@@ -157,7 +156,7 @@ proof -
         by typecheck_cfuncs
       show "right_cart_proj \<nat>\<^sub>c B \<circ>\<^sub>c y\<^sup>\<flat> : A \<times>\<^sub>c \<nat>\<^sub>c \<rightarrow> B"
         by typecheck_cfuncs
-      fix x 
+      fix x
       assume x_type[type_rule]: "x \<in>\<^sub>c A \<times>\<^sub>c \<nat>\<^sub>c"
       obtain a m where a_type[type_rule]: "a \<in>\<^sub>c A" and m_type[type_rule]: "m \<in>\<^sub>c \<nat>\<^sub>c"
         and x_def: "x = \<langle>a, m\<rangle>"
@@ -193,18 +192,549 @@ proof -
     qed
   qed
 qed
+
+
+
+theorem minimisation:
+  assumes f_type[type_rule]: "f : (\<nat>\<^sub>c \<times>\<^sub>c A) \<rightarrow> \<nat>\<^sub>c"
+  shows
+    "\<exists>! \<mu>. \<mu> : A \<rightarrow> (\<nat>\<^sub>c \<Coprod> \<one>) \<and>
+      (\<forall>a n. (a \<in>\<^sub>c A \<and> n \<in>\<^sub>c \<nat>\<^sub>c) \<longrightarrow>
+        (\<mu> \<circ>\<^sub>c a = (left_coproj \<nat>\<^sub>c \<one>) \<circ>\<^sub>c n \<longleftrightarrow>
+          (f \<circ>\<^sub>c \<langle>n, a\<rangle> = zero \<and>
+           (\<forall>m. m \<in>\<^sub>c \<nat>\<^sub>c \<longrightarrow> (m <\<^sub>\<nat> n \<longrightarrow> f \<circ>\<^sub>c \<langle>m, a\<rangle> \<noteq> zero))))) \<and>
+      (\<forall>a. a \<in>\<^sub>c A \<longrightarrow>
+        (\<mu> \<circ>\<^sub>c a = (right_coproj \<nat>\<^sub>c \<one>) \<circ>\<^sub>c id\<^sub>c \<one> \<longleftrightarrow>
+          (\<forall>n. n \<in>\<^sub>c \<nat>\<^sub>c \<longrightarrow> f \<circ>\<^sub>c \<langle>n, a\<rangle> \<noteq> zero)))"
+proof -
+
+  define zero_NA :: cfunc where
+    "zero_NA = zero \<circ>\<^sub>c \<beta>\<^bsub>\<nat>\<^sub>c \<times>\<^sub>c A\<^esub>"
+  have zero_NA_type[type_rule]: "zero_NA : (\<nat>\<^sub>c \<times>\<^sub>c A) \<rightarrow> \<nat>\<^sub>c"
+    unfolding zero_NA_def by typecheck_cfuncs
+
+  (*  Zf(n,a) :\<equiv> f(n,a)=0 --- *)
+  define Zf :: cfunc where
+    "Zf = eq_pred \<nat>\<^sub>c \<circ>\<^sub>c \<langle>f, zero_NA\<rangle>"
+  have Zf_type[type_rule]: "Zf : (\<nat>\<^sub>c \<times>\<^sub>c A) \<rightarrow> \<Omega>"
+    unfolding Zf_def by typecheck_cfuncs
+
+  (*  Pf(n,a) :\<equiv> f(n,a)\<noteq>0 --- *)
+  define Pf :: cfunc where
+    "Pf = NOT \<circ>\<^sub>c Zf"
+  have Pf_type[type_rule]: "Pf : (\<nat>\<^sub>c \<times>\<^sub>c A) \<rightarrow> \<Omega>"
+    unfolding Pf_def by typecheck_cfuncs
+
+  (*  P(m,(n,a)) :\<equiv> (m<n \<Rightarrow> Pf(m,a)) --- *)
+  obtain P  where
+    P_def: "P =
+      IMPLIES \<circ>\<^sub>c
+        \<langle> lt \<circ>\<^sub>c
+            \<langle> left_cart_proj \<nat>\<^sub>c (\<nat>\<^sub>c \<times>\<^sub>c A),
+              left_cart_proj \<nat>\<^sub>c A \<circ>\<^sub>c right_cart_proj \<nat>\<^sub>c (\<nat>\<^sub>c \<times>\<^sub>c A) \<rangle>,
+          Pf \<circ>\<^sub>c
+            \<langle> left_cart_proj \<nat>\<^sub>c (\<nat>\<^sub>c \<times>\<^sub>c A),
+              right_cart_proj \<nat>\<^sub>c A \<circ>\<^sub>c right_cart_proj \<nat>\<^sub>c (\<nat>\<^sub>c \<times>\<^sub>c A) \<rangle> \<rangle>"  
+    by blast
+  then have P_type[type_rule]: "P : (\<nat>\<^sub>c \<times>\<^sub>c (\<nat>\<^sub>c \<times>\<^sub>c A)) \<rightarrow> \<Omega>"
+    unfolding P_def  
+    by (typecheck_cfuncs,
+        smt (verit, ccfv_SIG) NOT_type comp_type leq_type lt_def swap_def swap_type)
+
+ 
+    (*  Curry in m to get Psharp : (\<nat>\<times>A) \<rightarrow> \<Omega>^\<nat> --- *)
+  obtain Psharp where
+    Psharp_def: "Psharp = P\<^sup>\<sharp>"
+    by blast
+  then have Psharp_type[type_rule]: "Psharp : (\<nat>\<^sub>c \<times>\<^sub>c A) \<rightarrow> \<Omega>\<^bsup>\<nat>\<^sub>c\<^esup>"
+    unfolding Psharp_def
+    by typecheck_cfuncs
+
+  (*  \<chi>_f(n,a) :\<equiv> Zf(n,a) \<and> \<forall>m. P(m,n,a) --- *)
+  obtain chi_f where
+    chi_f_def: "chi_f = AND \<circ>\<^sub>c \<langle> Zf, (FORALL \<nat>\<^sub>c) \<circ>\<^sub>c Psharp \<rangle>"
+    by blast
+  then have chi_f_type[type_rule]: "chi_f : (\<nat>\<^sub>c \<times>\<^sub>c A) \<rightarrow> \<Omega>"
+    unfolding chi_f_def
+    by typecheck_cfuncs
+
+
+  obtain exists_f where
+    exists_f_def: "exists_f = (EXISTS \<nat>\<^sub>c) \<circ>\<^sub>c (chi_f\<^sup>\<sharp>)"
+    by blast
+  then have exists_f_type[type_rule]: "exists_f : A \<rightarrow> \<Omega>"
+    unfolding exists_f_def
+    by typecheck_cfuncs
+
+   have chi_f_sharp_type[type_rule]: "chi_f\<^sup>\<sharp> : A \<rightarrow> \<Omega>\<^bsup>\<nat>\<^sub>c\<^esup>"
+    by (simp add: chi_f_type transpose_func_type)
+
+
+
+  have exists_f_semantics:
+  "\<And>a. a \<in>\<^sub>c A \<Longrightarrow>
+     exists_f \<circ>\<^sub>c a = \<t> \<longleftrightarrow> (\<exists>n. n \<in>\<^sub>c \<nat>\<^sub>c \<and> chi_f \<circ>\<^sub>c \<langle>n, a\<rangle> = \<t>)"
+  proof safe
+    fix a
+    assume a_type[type_rule]: "a \<in>\<^sub>c A"
+    assume LHS: "exists_f \<circ>\<^sub>c a = \<t>"
+    then have exists: "(EXISTS \<nat>\<^sub>c) \<circ>\<^sub>c  chi_f\<^sup>\<sharp> \<circ>\<^sub>c a = \<t>"
+      using comp_associative2 exists_f_def by (typecheck_cfuncs, auto)
+    have "(chi_f\<^sup>\<sharp> \<circ>\<^sub>c a) = (chi_f \<circ>\<^sub>c \<langle>id \<nat>\<^sub>c, a  \<circ>\<^sub>c \<beta>\<^bsub>\<nat>\<^sub>c\<^esub>\<rangle> \<circ>\<^sub>c left_cart_proj \<nat>\<^sub>c \<one>)\<^sup>\<sharp>"
+    proof -  
+      have "(chi_f\<^sup>\<sharp> \<circ>\<^sub>c a)\<^sup>\<flat>  = ((chi_f\<^sup>\<sharp>)\<^sup>\<flat> \<circ>\<^sub>c (id \<nat>\<^sub>c \<times>\<^sub>f a))"
+        by (typecheck_cfuncs, simp add: inv_transpose_of_composition)
+      also have "... = (chi_f \<circ>\<^sub>c (id \<nat>\<^sub>c \<times>\<^sub>f a))"
+        using chi_f_type flat_cancels_sharp by auto
+      also have "... = chi_f \<circ>\<^sub>c \<langle>id \<nat>\<^sub>c \<circ>\<^sub>c left_cart_proj \<nat>\<^sub>c \<one>, a \<circ>\<^sub>c right_cart_proj \<nat>\<^sub>c \<one>\<rangle>"
+        by (typecheck_cfuncs, simp add: cfunc_cross_prod_def2)
+      also have "... = chi_f \<circ>\<^sub>c \<langle>id \<nat>\<^sub>c \<circ>\<^sub>c left_cart_proj \<nat>\<^sub>c \<one>, (a \<circ>\<^sub>c \<beta>\<^bsub>\<nat>\<^sub>c\<^esub>) \<circ>\<^sub>c left_cart_proj \<nat>\<^sub>c \<one>\<rangle>"        
+        by (etcs_assocr, typecheck_cfuncs, metis terminal_func_unique)
+      also have "... = (chi_f \<circ>\<^sub>c \<langle>id \<nat>\<^sub>c, a \<circ>\<^sub>c \<beta>\<^bsub>\<nat>\<^sub>c\<^esub>\<rangle>) \<circ>\<^sub>c left_cart_proj \<nat>\<^sub>c \<one>"
+        by (etcs_assocr, typecheck_cfuncs, simp add: cfunc_prod_comp comp_associative2)
+      finally show ?thesis
+        using cfunc_cross_prod_right_terminal_decomp sharp_comp by (typecheck_cfuncs, force)
+    qed
+    then have "(EXISTS \<nat>\<^sub>c) \<circ>\<^sub>c  (chi_f \<circ>\<^sub>c \<langle>id \<nat>\<^sub>c, a  \<circ>\<^sub>c \<beta>\<^bsub>\<nat>\<^sub>c\<^esub>\<rangle> \<circ>\<^sub>c left_cart_proj \<nat>\<^sub>c \<one>)\<^sup>\<sharp> = \<t>"
+      using exists by argo
+    then have "\<exists> n. n \<in>\<^sub>c \<nat>\<^sub>c \<and> (chi_f \<circ>\<^sub>c \<langle>id \<nat>\<^sub>c, a  \<circ>\<^sub>c \<beta>\<^bsub>\<nat>\<^sub>c\<^esub>\<rangle>) \<circ>\<^sub>c n = \<t>"
+      by (typecheck_cfuncs,
+          smt (verit, best) EXISTS_true_implies_exists_true comp_associative2 left_cart_proj_type)
+    then show "\<exists>n. n \<in>\<^sub>c \<nat>\<^sub>c \<and> chi_f \<circ>\<^sub>c \<langle>n,a\<rangle> = \<t>"
+      using right_param_def2 right_param_on_el by (typecheck_cfuncs, auto)
+  next
+    fix a n
+    assume a_type[type_rule]: "a \<in>\<^sub>c A"
+    assume n_type[type_rule]: "n \<in>\<^sub>c \<nat>\<^sub>c"
+    assume RHS: "chi_f \<circ>\<^sub>c \<langle>n,a\<rangle> = \<t>"
+
+    let ?p = "chi_f \<circ>\<^sub>c \<langle>id \<nat>\<^sub>c, a \<circ>\<^sub>c \<beta>\<^bsub>\<nat>\<^sub>c\<^esub>\<rangle>"
+    have p_type[type_rule]: "?p : \<nat>\<^sub>c \<rightarrow> \<Omega>"
+      by typecheck_cfuncs
+
+    have p_at_n: "?p \<circ>\<^sub>c n = \<t>"
+      using RHS
+      by (typecheck_cfuncs, metis right_param_def2 right_param_on_el)
+
+    have ex_p_true: "\<exists>x. x \<in>\<^sub>c \<nat>\<^sub>c \<and> ?p \<circ>\<^sub>c x = \<t>"
+      using n_type p_at_n by blast
+
+    have EXISTS_p_true:
+      "(EXISTS \<nat>\<^sub>c) \<circ>\<^sub>c (?p \<circ>\<^sub>c left_cart_proj \<nat>\<^sub>c \<one>)\<^sup>\<sharp> = \<t>"
+      using exists_true_implies_EXISTS_true[OF p_type ex_p_true].
+
+    have chi_sharp_a:
+      "chi_f\<^sup>\<sharp> \<circ>\<^sub>c a = (?p \<circ>\<^sub>c left_cart_proj \<nat>\<^sub>c \<one>)\<^sup>\<sharp>"
+      by (typecheck_cfuncs, smt (verit, ccfv_SIG)
+          cfunc_cross_prod_right_terminal_decomp comp_associative2 sharp_comp)
+   
+    then have EXISTS_chi_true:
+      "(EXISTS \<nat>\<^sub>c) \<circ>\<^sub>c (chi_f\<^sup>\<sharp> \<circ>\<^sub>c a) = \<t>"
+      using EXISTS_p_true by simp
+
+
+    show "exists_f \<circ>\<^sub>c a = \<t>"
+      unfolding exists_f_def
+      using EXISTS_chi_true
+      by (typecheck_cfuncs, simp add: comp_associative2)
+  qed
+ 
+  have chi_f_functional:
+    "\<And>a n1 n2. a \<in>\<^sub>c A \<Longrightarrow> n1 \<in>\<^sub>c \<nat>\<^sub>c \<Longrightarrow> n2 \<in>\<^sub>c \<nat>\<^sub>c \<Longrightarrow>
+      chi_f \<circ>\<^sub>c \<langle>n1,a\<rangle> = \<t> \<Longrightarrow> chi_f \<circ>\<^sub>c \<langle>n2,a\<rangle> = \<t> \<Longrightarrow> n1 = n2"
+  proof -
+    fix a n1 n2
+    assume aA[type_rule]: "a \<in>\<^sub>c A"
+     assume n1N[type_rule]: "n1 \<in>\<^sub>c \<nat>\<^sub>c"
+     assume n2N[type_rule]: "n2 \<in>\<^sub>c \<nat>\<^sub>c"
+     assume chi1: "chi_f \<circ>\<^sub>c \<langle>n1,a\<rangle> = \<t>"
+     assume chi2: "chi_f \<circ>\<^sub>c \<langle>n2,a\<rangle> = \<t>"
+     
+     (* --- unpack chi_f at (n1,a)  --- *)
+     have f1: "Zf \<circ>\<^sub>c \<langle>n1,a\<rangle> = \<t> \<and> (FORALL \<nat>\<^sub>c) \<circ>\<^sub>c Psharp \<circ>\<^sub>c \<langle>n1,a\<rangle> = \<t>"
+     proof -
+       have "(AND \<circ>\<^sub>c \<langle>Zf, (FORALL \<nat>\<^sub>c) \<circ>\<^sub>c Psharp\<rangle>) \<circ>\<^sub>c \<langle>n1,a\<rangle> = \<t>"
+         using chi1 chi_f_def by auto
+       then have "AND \<circ>\<^sub>c \<langle>Zf \<circ>\<^sub>c \<langle>n1,a\<rangle>, (FORALL \<nat>\<^sub>c) \<circ>\<^sub>c Psharp \<circ>\<^sub>c \<langle>n1,a\<rangle>\<rangle>  = \<t>"
+         by (typecheck_cfuncs, smt (z3) cfunc_prod_comp cfunc_prod_type comp_associative2 comp_type)
+       then show ?thesis
+         by (typecheck_cfuncs, meson AND_true_imp_both_true)
+     qed
   
-      
-              
+     (* --- unpack chi_f at (n2,a)  --- *)
+     have f2: "Zf \<circ>\<^sub>c \<langle>n2,a\<rangle> = \<t> \<and> (FORALL \<nat>\<^sub>c) \<circ>\<^sub>c Psharp \<circ>\<^sub>c \<langle>n2,a\<rangle> = \<t>"
+     proof -
+       have "(AND \<circ>\<^sub>c \<langle>Zf, (FORALL \<nat>\<^sub>c) \<circ>\<^sub>c Psharp\<rangle>) \<circ>\<^sub>c \<langle>n2,a\<rangle> = \<t>"
+         using chi2 chi_f_def by auto
+       then have "AND \<circ>\<^sub>c \<langle>Zf \<circ>\<^sub>c \<langle>n2,a\<rangle>, (FORALL \<nat>\<^sub>c) \<circ>\<^sub>c Psharp \<circ>\<^sub>c \<langle>n2,a\<rangle>\<rangle>  = \<t>"
+         by (etcs_assocl, typecheck_cfuncs, smt (verit, ccfv_SIG)  cfunc_prod_comp cfunc_prod_type
+             comp_associative2)
+       then show ?thesis
+         by (typecheck_cfuncs, meson AND_true_imp_both_true)
+     qed
+  
+     have "(leq \<circ>\<^sub>c \<langle>n1, n2\<rangle> = \<t>) \<or> (leq \<circ>\<^sub>c \<langle>n2, n1\<rangle> = \<t>)"
+       by (simp add: lqe_connexity n1N n2N)
+      (* --- trichotomy on n1,n2 --- *)
+     then have tri: "n1 = n2 \<or> n1 <\<^sub>\<nat> n2 \<or> n2 <\<^sub>\<nat> n1"
+       by (simp add: lt_trichotomy n1N n2N)
+     show "n1 = n2"
+     proof (rule disjE[OF tri])
+       assume "n1 = n2"
+       then show "n1 = n2".
+     next
+       assume dichotomy: "n1 <\<^sub>\<nat> n2 \<or> n2 <\<^sub>\<nat> n1"
+       show "n1 = n2"
+       proof(cases "n1 <\<^sub>\<nat> n2")
+          assume lt12: "n1 <\<^sub>\<nat> n2"
+     
+          (* From For2 we will extract P(n1,(n2,a)) = \<t>, i.e. (n1<n2 \<Rightarrow> Pf(n1,a)) *)
+          define p2 :: cfunc where
+            "p2 = P \<circ>\<^sub>c \<langle> id \<nat>\<^sub>c, (\<langle>n2,a\<rangle> \<circ>\<^sub>c \<beta>\<^bsub>\<nat>\<^sub>c\<^esub>) \<rangle>"
+          have p2_type[type_rule]: "p2 : \<nat>\<^sub>c \<rightarrow> \<Omega>"
+            unfolding p2_def by typecheck_cfuncs
+     
+          (* Key typing/transpose fact: Psharp \<circ> \<langle>n2,a\<rangle> is the curry of p2\<circ>\<pi>0 *)
+          have curry_id:
+            "Psharp \<circ>\<^sub>c \<langle>n2,a\<rangle> = (p2 \<circ>\<^sub>c left_cart_proj \<nat>\<^sub>c \<one>)\<^sup>\<sharp>"
+          proof -
+            (* prove by showing their flats are equal *)
+            have flat_eq:
+              "(Psharp \<circ>\<^sub>c \<langle>n2,a\<rangle>)\<^sup>\<flat> = p2 \<circ>\<^sub>c left_cart_proj \<nat>\<^sub>c \<one>"
+            proof -
+              have "(Psharp \<circ>\<^sub>c \<langle>n2,a\<rangle>)\<^sup>\<flat> = Psharp\<^sup>\<flat> \<circ>\<^sub>c (id \<nat>\<^sub>c \<times>\<^sub>f \<langle>n2,a\<rangle>)"
+                by (typecheck_cfuncs, simp add: inv_transpose_of_composition)
+              also have "... = P \<circ>\<^sub>c (id \<nat>\<^sub>c \<times>\<^sub>f \<langle>n2,a\<rangle>)"
+                using P_type Psharp_def flat_cancels_sharp by moura
+  
+              also have "... = P \<circ>\<^sub>c \<langle> id \<nat>\<^sub>c \<circ>\<^sub>c left_cart_proj \<nat>\<^sub>c \<one>,
+                                     \<langle>n2,a\<rangle> \<circ>\<^sub>c right_cart_proj \<nat>\<^sub>c \<one> \<rangle>"
+                by (typecheck_cfuncs, simp add: cfunc_cross_prod_def2)
+              also have "... = P \<circ>\<^sub>c \<langle> id \<nat>\<^sub>c \<circ>\<^sub>c left_cart_proj \<nat>\<^sub>c \<one>,
+                                     (\<langle>n2,a\<rangle> \<circ>\<^sub>c \<beta>\<^bsub>\<nat>\<^sub>c\<^esub>) \<circ>\<^sub>c left_cart_proj \<nat>\<^sub>c \<one> \<rangle>"
+                by (etcs_assocr, typecheck_cfuncs, metis terminal_func_unique)
+              also have "... = (P \<circ>\<^sub>c \<langle> id \<nat>\<^sub>c, (\<langle>n2,a\<rangle> \<circ>\<^sub>c \<beta>\<^bsub>\<nat>\<^sub>c\<^esub>) \<rangle>) \<circ>\<^sub>c left_cart_proj \<nat>\<^sub>c \<one>"
+                by (etcs_assocr, typecheck_cfuncs, simp add: cfunc_prod_comp comp_associative2)
+              also have "... = p2 \<circ>\<^sub>c left_cart_proj \<nat>\<^sub>c \<one>"
+                unfolding p2_def by simp
+              finally show ?thesis .
+            qed
+            show ?thesis
+              by (metis Psharp_type aA cfunc_prod_type comp_type flat_eq n2N sharp_cancels_flat)
+          qed
+  
+          have For2': "(FORALL \<nat>\<^sub>c) \<circ>\<^sub>c (p2 \<circ>\<^sub>c left_cart_proj \<nat>\<^sub>c \<one>)\<^sup>\<sharp> = \<t>"
+            using curry_id f2 by presburger
+  
+  
+          have P_at_n1: "p2 \<circ>\<^sub>c n1 = \<t>"
+            using FORALL_true_implies_all_true curry_id f2 n1N p2_type by presburger
+  
+          have P_pair: "P \<circ>\<^sub>c \<langle>n1, \<langle>n2,a\<rangle>\<rangle> = \<t>"
+            using P_at_n1
+            unfolding p2_def
+            by (smt (verit, ccfv_SIG) P_type aA cart_prod_extract_left cfunc_prod_type
+                comp_associative2 comp_type id_type n1N n2N terminal_func_type)
+  
+  
+         (* Unfold P: with lt(n1,n2)=\<t>, IMPLIES forces Pf(n1,a)=\<t> *)
+          have lt_comp: "lt \<circ>\<^sub>c \<langle>n1,n2\<rangle> = \<t>"
+            using lt12 unfolding lt_infix_def by simp
+  
+          have Zf1: "Zf \<circ>\<^sub>c \<langle>n1,a\<rangle> = \<t>"
+            using f1 by simp
+  
+          have Pf1_false: "Pf \<circ>\<^sub>c \<langle>n1,a\<rangle> = \<f>"
+          proof -
+            have "Pf \<circ>\<^sub>c \<langle>n1,a\<rangle> = (NOT \<circ>\<^sub>c Zf) \<circ>\<^sub>c \<langle>n1,a\<rangle>"
+              using Pf_def by fastforce
+            also have "... = NOT \<circ>\<^sub>c (Zf \<circ>\<^sub>c \<langle>n1,a\<rangle>)"
+              by (typecheck_cfuncs, simp add: comp_associative2)
+            also have "... = NOT \<circ>\<^sub>c \<t>"
+              using Zf1 by simp
+            also have "... = \<f>"
+              using NOT_true_is_false by blast
+            finally show ?thesis.
+          qed
+  
+          then have "NOT \<circ>\<^sub>c Pf = Zf"
+            using NOT_type Pf_def Zf_type comp_associative2 double_negation id_left_unit2 by auto
+  
+          have Pf1_true: "Pf \<circ>\<^sub>c \<langle>n1,a\<rangle> = \<t>"
+          proof -
+            have P_pair_unfold:
+              "P \<circ>\<^sub>c \<langle>n1, \<langle>n2,a\<rangle>\<rangle>
+               =
+               IMPLIES \<circ>\<^sub>c
+        \<langle> lt \<circ>\<^sub>c
+            \<langle> left_cart_proj \<nat>\<^sub>c (\<nat>\<^sub>c \<times>\<^sub>c A),
+              left_cart_proj \<nat>\<^sub>c A \<circ>\<^sub>c right_cart_proj \<nat>\<^sub>c (\<nat>\<^sub>c \<times>\<^sub>c A) \<rangle>,
+          Pf \<circ>\<^sub>c
+            \<langle> left_cart_proj \<nat>\<^sub>c (\<nat>\<^sub>c \<times>\<^sub>c A),
+              right_cart_proj \<nat>\<^sub>c A \<circ>\<^sub>c right_cart_proj \<nat>\<^sub>c (\<nat>\<^sub>c \<times>\<^sub>c A) \<rangle> \<rangle> \<circ>\<^sub>c \<langle>n1, \<langle>n2,a\<rangle>\<rangle>"
+              unfolding P_def
+              by (typecheck_cfuncs, smt (verit) NOT_type comp_associative2
+                    comp_type leq_type lt_def swap_def swap_type)
+            also have " ... = IMPLIES \<circ>\<^sub>c
+        \<langle> lt \<circ>\<^sub>c
+            \<langle> left_cart_proj \<nat>\<^sub>c (\<nat>\<^sub>c \<times>\<^sub>c A),
+              left_cart_proj \<nat>\<^sub>c A \<circ>\<^sub>c right_cart_proj \<nat>\<^sub>c (\<nat>\<^sub>c \<times>\<^sub>c A) \<rangle> \<circ>\<^sub>c \<langle>n1, \<langle>n2,a\<rangle>\<rangle>,
+          Pf \<circ>\<^sub>c
+            \<langle> left_cart_proj \<nat>\<^sub>c (\<nat>\<^sub>c \<times>\<^sub>c A),
+              right_cart_proj \<nat>\<^sub>c A \<circ>\<^sub>c right_cart_proj \<nat>\<^sub>c (\<nat>\<^sub>c \<times>\<^sub>c A) \<rangle> \<circ>\<^sub>c \<langle>n1, \<langle>n2,a\<rangle>\<rangle> \<rangle>"
+              by (typecheck_cfuncs, smt (verit) NOT_type cfunc_prod_comp cfunc_type_def
+                    comp_associative comp_type leq_type lt_def swap_def swap_type)
+            also have " ... = IMPLIES \<circ>\<^sub>c
+        \<langle> lt \<circ>\<^sub>c
+            \<langle> left_cart_proj \<nat>\<^sub>c (\<nat>\<^sub>c \<times>\<^sub>c A) \<circ>\<^sub>c \<langle>n1, \<langle>n2,a\<rangle>\<rangle>,
+              left_cart_proj \<nat>\<^sub>c A \<circ>\<^sub>c right_cart_proj \<nat>\<^sub>c (\<nat>\<^sub>c \<times>\<^sub>c A) \<circ>\<^sub>c \<langle>n1, \<langle>n2,a\<rangle>\<rangle>\<rangle>,
+          Pf \<circ>\<^sub>c
+            \<langle> left_cart_proj \<nat>\<^sub>c (\<nat>\<^sub>c \<times>\<^sub>c A) \<circ>\<^sub>c \<langle>n1, \<langle>n2,a\<rangle>\<rangle>,
+              right_cart_proj \<nat>\<^sub>c A \<circ>\<^sub>c right_cart_proj \<nat>\<^sub>c (\<nat>\<^sub>c \<times>\<^sub>c A) \<circ>\<^sub>c \<langle>n1, \<langle>n2,a\<rangle>\<rangle> \<rangle> \<rangle>"
+              using cfunc_prod_comp comp_associative2 by (typecheck_cfuncs, auto)
+            also have " ... = IMPLIES \<circ>\<^sub>c
+          \<langle> lt \<circ>\<^sub>c
+              \<langle> left_cart_proj \<nat>\<^sub>c (\<nat>\<^sub>c \<times>\<^sub>c A) \<circ>\<^sub>c \<langle>n1, \<langle>n2,a\<rangle>\<rangle>,
+                left_cart_proj \<nat>\<^sub>c A \<circ>\<^sub>c \<langle>n2,a\<rangle>\<rangle>,
+            Pf \<circ>\<^sub>c
+              \<langle> left_cart_proj \<nat>\<^sub>c (\<nat>\<^sub>c \<times>\<^sub>c A) \<circ>\<^sub>c \<langle>n1, \<langle>n2,a\<rangle>\<rangle>,
+                right_cart_proj \<nat>\<^sub>c A \<circ>\<^sub>c \<langle>n2,a\<rangle> \<rangle> \<rangle>"
+              by (typecheck_cfuncs, metis right_cart_proj_cfunc_prod)
+            also have " ... = IMPLIES \<circ>\<^sub>c \<langle> lt \<circ>\<^sub>c \<langle> n1, n2\<rangle>, Pf \<circ>\<^sub>c \<langle> n1, a\<rangle>\<rangle>"
+              by (typecheck_cfuncs, metis left_cart_proj_cfunc_prod right_cart_proj_cfunc_prod)
+            also have " ... = IMPLIES \<circ>\<^sub>c \<langle> lt \<circ>\<^sub>c \<langle> n1, n2\<rangle>, \<t>\<rangle>"
+              by (typecheck_cfuncs, metis IMPLIES_true_true_is_true P_pair calculation lt12 lt_infix_def)
+            also have "... = \<t>"
+              using P_pair calculation by argo
+            finally show ?thesis
+              using IMPLIES_true_false_is_false IMPLIES_true_true_is_true Pf1_false
+                \<open>IMPLIES \<circ>\<^sub>c \<langle>lt \<circ>\<^sub>c \<langle>n1,n2\<rangle>,Pf \<circ>\<^sub>c \<langle>n1,a\<rangle>\<rangle> = IMPLIES \<circ>\<^sub>c \<langle>lt \<circ>\<^sub>c \<langle>n1,n2\<rangle>,\<t>\<rangle>\<close> lt_comp by argo              
+          qed
+  
+          then show "n1 = n2"
+            using Pf1_false true_false_distinct by auto          
+      next
+        assume "\<not> n1 <\<^sub>\<nat> n2"
+        then have lt21: "n2 <\<^sub>\<nat> n1"
+          using dichotomy by blast
+  
+        (* symmetric to the previous case: swap (n1,n2) and use For1 instead of For2 *)
+        define p1 :: cfunc where
+          "p1 = P \<circ>\<^sub>c \<langle> id \<nat>\<^sub>c, (\<langle>n1,a\<rangle> \<circ>\<^sub>c \<beta>\<^bsub>\<nat>\<^sub>c\<^esub>) \<rangle>"
+        have p1_type[type_rule]: "p1 : \<nat>\<^sub>c \<rightarrow> \<Omega>"
+          unfolding p1_def by typecheck_cfuncs
+  
+        have curry_id':
+          "Psharp \<circ>\<^sub>c \<langle>n1,a\<rangle> = (p1 \<circ>\<^sub>c left_cart_proj \<nat>\<^sub>c \<one>)\<^sup>\<sharp>"
+        proof -
+          (* prove by showing their flats are equal *)
+          have flat_eq:
+            "(Psharp \<circ>\<^sub>c \<langle>n1,a\<rangle>)\<^sup>\<flat> = p1 \<circ>\<^sub>c left_cart_proj \<nat>\<^sub>c \<one>"
+          proof -
+            have "(Psharp \<circ>\<^sub>c \<langle>n1,a\<rangle>)\<^sup>\<flat> = Psharp\<^sup>\<flat> \<circ>\<^sub>c (id \<nat>\<^sub>c \<times>\<^sub>f \<langle>n1,a\<rangle>)"
+              by (typecheck_cfuncs, simp add: inv_transpose_of_composition)
+            also have "... = P \<circ>\<^sub>c (id \<nat>\<^sub>c \<times>\<^sub>f \<langle>n1,a\<rangle>)"
+              using P_type Psharp_def flat_cancels_sharp by moura
+  
+            also have "... = P \<circ>\<^sub>c \<langle> id \<nat>\<^sub>c \<circ>\<^sub>c left_cart_proj \<nat>\<^sub>c \<one>,
+                                   \<langle>n1,a\<rangle> \<circ>\<^sub>c right_cart_proj \<nat>\<^sub>c \<one> \<rangle>"
+              by (typecheck_cfuncs, simp add: cfunc_cross_prod_def2)
+            also have "... = P \<circ>\<^sub>c \<langle> id \<nat>\<^sub>c \<circ>\<^sub>c left_cart_proj \<nat>\<^sub>c \<one>,
+                                   (\<langle>n1,a\<rangle> \<circ>\<^sub>c \<beta>\<^bsub>\<nat>\<^sub>c\<^esub>) \<circ>\<^sub>c left_cart_proj \<nat>\<^sub>c \<one> \<rangle>"
+              by (etcs_assocr, typecheck_cfuncs, metis terminal_func_unique)
+            also have "... = (P \<circ>\<^sub>c \<langle> id \<nat>\<^sub>c, (\<langle>n1,a\<rangle> \<circ>\<^sub>c \<beta>\<^bsub>\<nat>\<^sub>c\<^esub>) \<rangle>) \<circ>\<^sub>c left_cart_proj \<nat>\<^sub>c \<one>"
+              by (etcs_assocr, typecheck_cfuncs, simp add: cfunc_prod_comp comp_associative2)
+            also have "... = p1 \<circ>\<^sub>c left_cart_proj \<nat>\<^sub>c \<one>"
+              unfolding p1_def by simp
+            finally show ?thesis.
+          qed
+          show ?thesis
+            by (metis Psharp_type aA cfunc_prod_type comp_type flat_eq n1N sharp_cancels_flat)
+        qed
+        have For1': "(FORALL \<nat>\<^sub>c) \<circ>\<^sub>c (p1 \<circ>\<^sub>c left_cart_proj \<nat>\<^sub>c \<one>)\<^sup>\<sharp> = \<t>"
+            using curry_id' f1 by presburger
+   
+        have P_at_n2: "p1 \<circ>\<^sub>c n2 = \<t>"
+          using FORALL_true_implies_all_true For1' n2N p1_type by blast
+  
+        have P_pair': "P \<circ>\<^sub>c \<langle>n2, \<langle>n1,a\<rangle>\<rangle> = \<t>"
+          using P_at_n2 P_type aA cfunc_prod_type n1N n2N p1_def
+                right_param_def2 right_param_on_el by auto
+        have lt_comp': "lt \<circ>\<^sub>c \<langle>n2,n1\<rangle> = \<t>"
+          using lt21 unfolding lt_infix_def by simp
+   
+        have Pf2: "Pf \<circ>\<^sub>c \<langle>n2,a\<rangle> = \<f>"
+        proof -
+          have "Pf \<circ>\<^sub>c \<langle>n2,a\<rangle> = (NOT \<circ>\<^sub>c Zf) \<circ>\<^sub>c \<langle>n2,a\<rangle>"
+            by (simp add: Pf_def)    
+          also have "... = NOT \<circ>\<^sub>c (Zf \<circ>\<^sub>c \<langle>n2,a\<rangle>)"
+            by (typecheck_cfuncs, simp add: comp_associative2)
+          also have "... = NOT \<circ>\<^sub>c \<t>"
+            using f2 by auto              
+          also have "... = \<f>"
+            using NOT_true_is_false by blast
+          finally show ?thesis.
+        qed
+  
+                  (* Unfold P at \<langle>n2,\<langle>n1,a\<rangle>\<rangle> to expose the IMPLIES structure *)
+        have P_pair_unfold:
+          "P \<circ>\<^sub>c \<langle>n2, \<langle>n1,a\<rangle>\<rangle>
+           = IMPLIES \<circ>\<^sub>c \<langle> lt \<circ>\<^sub>c \<langle>n2,n1\<rangle>, Pf \<circ>\<^sub>c \<langle>n2,a\<rangle> \<rangle>"
+        proof -
+          have "P \<circ>\<^sub>c \<langle>n2, \<langle>n1,a\<rangle>\<rangle> =
+          IMPLIES \<circ>\<^sub>c
+                  \<langle> lt \<circ>\<^sub>c
+                      \<langle> left_cart_proj \<nat>\<^sub>c (\<nat>\<^sub>c \<times>\<^sub>c A),
+                        left_cart_proj \<nat>\<^sub>c A \<circ>\<^sub>c right_cart_proj \<nat>\<^sub>c (\<nat>\<^sub>c \<times>\<^sub>c A) \<rangle>,
+                    Pf \<circ>\<^sub>c
+                      \<langle> left_cart_proj \<nat>\<^sub>c (\<nat>\<^sub>c \<times>\<^sub>c A),
+                        right_cart_proj \<nat>\<^sub>c A \<circ>\<^sub>c right_cart_proj \<nat>\<^sub>c (\<nat>\<^sub>c \<times>\<^sub>c A) \<rangle> \<rangle> \<circ>\<^sub>c \<langle>n2, \<langle>n1,a\<rangle>\<rangle>"
+            by (typecheck_cfuncs, smt (verit, ccfv_SIG) NOT_type P_def cfunc_type_def
+                comp_associative comp_type leq_type lt_def swap_def swap_type)
+          also have "... =  IMPLIES \<circ>\<^sub>c
+                  \<langle> lt \<circ>\<^sub>c
+                      \<langle> left_cart_proj \<nat>\<^sub>c (\<nat>\<^sub>c \<times>\<^sub>c A),
+                        left_cart_proj \<nat>\<^sub>c A \<circ>\<^sub>c right_cart_proj \<nat>\<^sub>c (\<nat>\<^sub>c \<times>\<^sub>c A) \<rangle>\<circ>\<^sub>c \<langle>n2, \<langle>n1,a\<rangle>\<rangle>,
+                    Pf \<circ>\<^sub>c
+                      \<langle> left_cart_proj \<nat>\<^sub>c (\<nat>\<^sub>c \<times>\<^sub>c A),
+                        right_cart_proj \<nat>\<^sub>c A \<circ>\<^sub>c right_cart_proj \<nat>\<^sub>c (\<nat>\<^sub>c \<times>\<^sub>c A) \<rangle> \<circ>\<^sub>c \<langle>n2, \<langle>n1,a\<rangle>\<rangle>\<rangle>"
+            by (typecheck_cfuncs, smt (verit) NOT_type cfunc_prod_comp cfunc_type_def
+                                  comp_associative comp_type leq_type lt_def swap_def swap_type)                
+          also have "... =  IMPLIES \<circ>\<^sub>c
+                  \<langle> lt \<circ>\<^sub>c
+                      \<langle> left_cart_proj \<nat>\<^sub>c (\<nat>\<^sub>c \<times>\<^sub>c A) \<circ>\<^sub>c \<langle>n2, \<langle>n1,a\<rangle>\<rangle>,
+                        left_cart_proj \<nat>\<^sub>c A \<circ>\<^sub>c right_cart_proj \<nat>\<^sub>c (\<nat>\<^sub>c \<times>\<^sub>c A) \<circ>\<^sub>c \<langle>n2, \<langle>n1,a\<rangle>\<rangle>\<rangle>,
+                    Pf \<circ>\<^sub>c
+                      \<langle> left_cart_proj \<nat>\<^sub>c (\<nat>\<^sub>c \<times>\<^sub>c A) \<circ>\<^sub>c \<langle>n2, \<langle>n1,a\<rangle>\<rangle> ,
+                        right_cart_proj \<nat>\<^sub>c A \<circ>\<^sub>c right_cart_proj \<nat>\<^sub>c (\<nat>\<^sub>c \<times>\<^sub>c A)\<circ>\<^sub>c \<langle>n2, \<langle>n1,a\<rangle>\<rangle> \<rangle> \<rangle>"
+            by (typecheck_cfuncs, simp add: cfunc_prod_comp comp_associative2)
+          also have "... =  IMPLIES \<circ>\<^sub>c
+                  \<langle> lt \<circ>\<^sub>c \<langle> n2, left_cart_proj \<nat>\<^sub>c A \<circ>\<^sub>c \<langle>n1,a\<rangle>\<rangle>,
+                    Pf \<circ>\<^sub>c \<langle> n2, right_cart_proj \<nat>\<^sub>c A \<circ>\<^sub>c \<langle>n1,a\<rangle> \<rangle> \<rangle>"
+            by (typecheck_cfuncs, simp add: left_cart_proj_cfunc_prod right_cart_proj_cfunc_prod)
+          also have "... =  IMPLIES \<circ>\<^sub>c \<langle> lt \<circ>\<^sub>c \<langle> n2, n1\<rangle>, Pf \<circ>\<^sub>c \<langle> n2, a \<rangle> \<rangle>"
+            using left_cart_proj_cfunc_prod right_cart_proj_cfunc_prod by (typecheck_cfuncs, auto)
+          finally show ?thesis.
+        qed
+  
+        have IMPL_t:
+          "IMPLIES \<circ>\<^sub>c \<langle> lt \<circ>\<^sub>c \<langle>n2,n1\<rangle>, Pf \<circ>\<^sub>c \<langle>n2,a\<rangle> \<rangle> = \<t>"
+          using P_pair' P_pair_unfold by simp
+  
+        have IMPL_f:
+          "IMPLIES \<circ>\<^sub>c \<langle> lt \<circ>\<^sub>c \<langle>n2,n1\<rangle>, Pf \<circ>\<^sub>c \<langle>n2,a\<rangle> \<rangle> = \<f>"
+        proof -
+          have "IMPLIES \<circ>\<^sub>c \<langle> lt \<circ>\<^sub>c \<langle>n2,n1\<rangle>, Pf \<circ>\<^sub>c \<langle>n2,a\<rangle> \<rangle>
+                = IMPLIES \<circ>\<^sub>c \<langle>\<t>, \<f>\<rangle>"
+            using lt_comp' Pf2 by simp
+          also have "... = \<f>"
+            using IMPLIES_true_false_is_false by simp
+          finally show ?thesis.
+        qed
+  
+        have False
+          using IMPL_f IMPL_t true_false_distinct by argo
+  
+        thus "n1 = n2"
+          by blast        
+      qed
+    qed
+  qed
 
+  thm equalizer_def
 
+  obtain M m where
+    m_equalizer: "equalizer M m chi_f (\<t> \<circ>\<^sub>c \<beta>\<^bsub>\<nat>\<^sub>c \<times>\<^sub>c A\<^esub>)"
+    using equalizer_exists by (typecheck_cfuncs, blast)
+  
+  have m_type[type_rule]: "m : M \<rightarrow> \<nat>\<^sub>c \<times>\<^sub>c A"
+    using cfunc_type_def chi_f_type equalizer_def m_equalizer
+    by presburger
 
+  have m_eq: "chi_f \<circ>\<^sub>c m = \<t> \<circ>\<^sub>c \<beta>\<^bsub>M\<^esub>"
+    using m_equalizer unfolding equalizer_def
+    by (-, typecheck_cfuncs, metis cfunc_type_def comp_associative
+        terminal_func_comp terminal_func_type true_func_type)
 
+  obtain D d where
+    d_equalizer: "equalizer D d exists_f (\<t> \<circ>\<^sub>c \<beta>\<^bsub>A\<^esub>)"
+    using equalizer_exists by (typecheck_cfuncs, blast)
 
+  have d_type[type_rule]: "d : D \<rightarrow> A"
+    using cfunc_type_def exists_f_type equalizer_def d_equalizer
+    by presburger
 
+  have d_monomorphism: "monomorphism d"
+    using d_equalizer equalizer_is_monomorphism by auto
+    
 
+  have d_eq: "exists_f \<circ>\<^sub>c d = \<t> \<circ>\<^sub>c \<beta>\<^bsub>D\<^esub>"
+    using d_equalizer unfolding equalizer_def
+    by (-, typecheck_cfuncs, metis cfunc_type_def comp_associative
+        terminal_func_comp terminal_func_type true_func_type)
 
+  have "exists_f \<circ>\<^sub>c right_cart_proj \<nat>\<^sub>c A \<circ>\<^sub>c m = \<t> \<circ>\<^sub>c \<beta>\<^bsub>A\<^esub> \<circ>\<^sub>c right_cart_proj \<nat>\<^sub>c A \<circ>\<^sub>c m"
+    sorry
+  then obtain e where 
+    e_type[type_rule]: "e: M \<rightarrow> D" and
+    e_d_eq: "d \<circ>\<^sub>c e = right_cart_proj \<nat>\<^sub>c A \<circ>\<^sub>c m"
+    using d_equalizer unfolding equalizer_def
+    by (-, typecheck_cfuncs, metis cfunc_type_def comp_associative)
 
+  have e_injective: "injective e"
+    sorry
+  have e_surjective: "surjective e"
+    sorry
+  have e_isomorphism: "isomorphism e"
+    sorry
 
+  define nu_f where "nu_f = left_cart_proj \<nat>\<^sub>c A \<circ>\<^sub>c m \<circ>\<^sub>c e\<^bold>\<inverse>"
+  have nu_f_type[type_rule]: "nu_f : D \<rightarrow> \<nat>\<^sub>c"
+    unfolding nu_f_def using e_isomorphism by typecheck_cfuncs
 
+  define mu_f where "mu_f = (nu_f \<bowtie>\<^sub>f \<beta>\<^bsub>A\<setminus>(D, d)\<^esub>) \<circ>\<^sub>c try_cast d"
+ 
+  show ?thesis
+  proof (rule ex1I[where a="mu_f"], safe)
+    show mu_f_type[type_rule]: "mu_f : A \<rightarrow> \<nat>\<^sub>c \<Coprod> \<one>"
+      unfolding mu_f_def using d_monomorphism by typecheck_cfuncs
 
+    show "\<And>a n. a \<in>\<^sub>c A \<Longrightarrow> n \<in>\<^sub>c \<nat>\<^sub>c \<Longrightarrow>
+           mu_f \<circ>\<^sub>c a = left_coproj \<nat>\<^sub>c \<one> \<circ>\<^sub>c n \<Longrightarrow>
+           f \<circ>\<^sub>c \<langle>n,a\<rangle> = zero"
+      sorry
+
+    show "\<And>a n m. a \<in>\<^sub>c A \<Longrightarrow> n \<in>\<^sub>c \<nat>\<^sub>c \<Longrightarrow>
+       mu_f \<circ>\<^sub>c a = left_coproj \<nat>\<^sub>c \<one> \<circ>\<^sub>c n \<Longrightarrow>
+       m \<in>\<^sub>c \<nat>\<^sub>c \<Longrightarrow> m <\<^sub>\<nat> n \<Longrightarrow> f \<circ>\<^sub>c \<langle>m,a\<rangle> = zero \<Longrightarrow> False"
+      sorry
+
+    show "\<And>a n. a \<in>\<^sub>c A \<Longrightarrow> n \<in>\<^sub>c \<nat>\<^sub>c \<Longrightarrow>
+           f \<circ>\<^sub>c \<langle>n,a\<rangle> = zero \<Longrightarrow>
+           \<forall>m. m \<in>\<^sub>c \<nat>\<^sub>c \<longrightarrow> m <\<^sub>\<nat> n \<longrightarrow> f \<circ>\<^sub>c \<langle>m,a\<rangle> \<noteq> zero \<Longrightarrow>
+           mu_f \<circ>\<^sub>c a = left_coproj \<nat>\<^sub>c \<one> \<circ>\<^sub>c n"
+      sorry
+
+    show "\<And>a n. a \<in>\<^sub>c A \<Longrightarrow>
+           mu_f \<circ>\<^sub>c a = right_coproj \<nat>\<^sub>c \<one> \<circ>\<^sub>c id\<^sub>c \<one> \<Longrightarrow>
+           n \<in>\<^sub>c \<nat>\<^sub>c \<Longrightarrow> f \<circ>\<^sub>c \<langle>n,a\<rangle> = zero \<Longrightarrow> False"
+      sorry
+
+    show "\<And>a. a \<in>\<^sub>c A \<Longrightarrow>
+         \<forall>n. n \<in>\<^sub>c \<nat>\<^sub>c \<longrightarrow> f \<circ>\<^sub>c \<langle>n,a\<rangle> \<noteq> zero \<Longrightarrow>
+         mu_f \<circ>\<^sub>c a = right_coproj \<nat>\<^sub>c \<one> \<circ>\<^sub>c id\<^sub>c \<one>"
+      sorry
+
+    show "\<And>\<mu>. \<mu> : A \<rightarrow> \<nat>\<^sub>c \<Coprod> \<one> \<Longrightarrow>
+         \<forall>a n. a \<in>\<^sub>c A \<and> n \<in>\<^sub>c \<nat>\<^sub>c \<longrightarrow>
+               (\<mu> \<circ>\<^sub>c a = left_coproj \<nat>\<^sub>c \<one> \<circ>\<^sub>c n) =
+               (f \<circ>\<^sub>c \<langle>n,a\<rangle> = zero \<and>
+                (\<forall>m. m \<in>\<^sub>c \<nat>\<^sub>c \<longrightarrow>
+                     m <\<^sub>\<nat> n \<longrightarrow> f \<circ>\<^sub>c \<langle>m,a\<rangle> \<noteq> zero)) \<Longrightarrow>
+         \<forall>a. a \<in>\<^sub>c A \<longrightarrow>
+             (\<mu> \<circ>\<^sub>c a = right_coproj \<nat>\<^sub>c \<one> \<circ>\<^sub>c id\<^sub>c \<one>) =
+             (\<forall>n. n \<in>\<^sub>c \<nat>\<^sub>c \<longrightarrow> f \<circ>\<^sub>c \<langle>n,a\<rangle> \<noteq> zero) \<Longrightarrow>
+         \<mu> = mu_f"
+      sorry
+  qed
+end
